theories/rules/rules_Jmp.v
@@ -5,7 +5,7 @@ From iris.proofmode Require Import tactics.
 From iris.algebra Require Import frac.
 
 Section cap_lang_rules.
-  Context `{memG Σ, regG Σ, MonRef: MonRefG (leibnizO _) CapR_rtc Σ}.
+  Context `{memG Σ, regG Σ}.
   Context `{MachineParameters}.
   Implicit Types P Q : iProp Σ.
   Implicit Types σ : ExecConf.
@@ -17,27 +17,24 @@ Section cap_lang_rules.
   Implicit Types reg : gmap RegName Word.
   Implicit Types ms : gmap Addr Word.
 
-  Lemma wp_jmp_success E pc_p pc_g pc_b pc_e pc_a w r w' pc_p':
+  Lemma wp_jmp_success E pc_p pc_b pc_e pc_a w r w' :
     decodeInstrW w = Jmp r →
-    PermFlows pc_p pc_p' →
-     isCorrectPC (inr ((pc_p,pc_g),pc_b,pc_e,pc_a)) →
+     isCorrectPC (inr (pc_p,pc_b,pc_e,pc_a)) →
 
-     {{{ ▷ PC ↦ᵣ inr ((pc_p,pc_g),pc_b,pc_e,pc_a)
-         ∗ ▷ pc_a ↦ₐ[pc_p'] w
+     {{{ ▷ PC ↦ᵣ inr (pc_p,pc_b,pc_e,pc_a)
+         ∗ ▷ pc_a ↦ₐ w
          ∗ ▷ r ↦ᵣ w' }}}
        Instr Executable @ E
        {{{ RET NextIV;
            PC ↦ᵣ updatePcPerm w'
-           ∗ pc_a ↦ₐ[pc_p'] w
+           ∗ pc_a ↦ₐ w
            ∗ r ↦ᵣ w' }}}.
   Proof.
-    iIntros (Hinstr Hfl Hvpc ϕ) "(>HPC & >Hpc_a & >Hr) Hφ".
+    iIntros (Hinstr Hvpc ϕ) "(>HPC & >Hpc_a & >Hr) Hφ".
     iApply wp_lift_atomic_head_step_no_fork; auto.
     iIntros (σ1 l1 l2 n) "Hσ1 /=". destruct σ1; simpl.
     iDestruct "Hσ1" as "[Hr0 Hm]".
-    assert (pc_p' ≠ O).
-    { destruct pc_p'; auto. destruct pc_p; inversion Hfl. inversion Hvpc; naive_solver. }
-    iDestruct (@gen_heap_valid_cap with "Hm Hpc_a") as %?; auto.
+    iDestruct (@gen_heap_valid with "Hm Hpc_a") as %?; auto.
     iDestruct (@gen_heap_valid with "Hr0 HPC") as %?.
     iDestruct (@gen_heap_valid with "Hr0 Hr") as %Hr_r0.
     iModIntro. iSplitR. by iPureIntro; apply normal_always_head_reducible.
@@ -50,25 +47,22 @@ Section cap_lang_rules.
     iApply "Hφ". iFrame. rewrite /RegLocate Hr_r0. eauto.
   Qed.
 
-  Lemma wp_jmp_successPC E pc_p pc_g pc_b pc_e pc_a w pc_p' :
+  Lemma wp_jmp_successPC E pc_p pc_b pc_e pc_a w :
     decodeInstrW w = Jmp PC →
-    PermFlows pc_p pc_p' →
-     isCorrectPC (inr ((pc_p,pc_g),pc_b,pc_e,pc_a)) →
+     isCorrectPC (inr (pc_p,pc_b,pc_e,pc_a)) →
 
-     {{{ ▷ PC ↦ᵣ inr ((pc_p,pc_g),pc_b,pc_e,pc_a)
-         ∗ ▷ pc_a ↦ₐ[pc_p'] w }}}
+     {{{ ▷ PC ↦ᵣ inr (pc_p,pc_b,pc_e,pc_a)
+         ∗ ▷ pc_a ↦ₐ w }}}
        Instr Executable @ E
        {{{ RET NextIV;
-           PC ↦ᵣ updatePcPerm (inr ((pc_p,pc_g),pc_b,pc_e,pc_a))
-           ∗ pc_a ↦ₐ[pc_p'] w }}}.
+           PC ↦ᵣ updatePcPerm (inr (pc_p,pc_b,pc_e,pc_a))
+           ∗ pc_a ↦ₐ w }}}.
   Proof.
-    iIntros (Hinstr Hfl Hvpc ϕ) "(>HPC & >Hpc_a) Hφ".
+    iIntros (Hinstr Hvpc ϕ) "(>HPC & >Hpc_a) Hφ".
     iApply wp_lift_atomic_head_step_no_fork; auto.
     iIntros (σ1 l1 l2 n) "Hσ1 /=". destruct σ1; cbn.
     iDestruct "Hσ1" as "[Hr0 Hm]".
-    assert (pc_p' ≠ O).
-    { destruct pc_p'; auto. destruct pc_p; inversion Hfl. inversion Hvpc; naive_solver. }
-    iDestruct (@gen_heap_valid_cap with "Hm Hpc_a") as %?; auto.
+    iDestruct (@gen_heap_valid with "Hm Hpc_a") as %?; auto.
     iDestruct (@gen_heap_valid with "Hr0 HPC") as %Hr_PC.
     iModIntro. iSplitR. by iPureIntro; apply normal_always_head_reducible.
     iNext. iIntros (e2 σ2 efs Hpstep).
