theories/rules/rules_Lea.v
@@ -5,7 +5,7 @@ From iris.proofmode Require Import tactics.
 From iris.algebra Require Import frac.
 
 Section cap_lang_rules.
-  Context `{HM: memG Σ, HR: regG Σ, MonRef: MonRefG (leibnizO _) CapR_rtc Σ}.
+  Context `{HM: memG Σ, HR: regG Σ}.
   Context `{MachineParameters}.
   Implicit Types P Q : iProp Σ.
   Implicit Types σ : ExecConf.
@@ -21,80 +21,64 @@ Section cap_lang_rules.
   | Lea_fail_rv_nonconst :
      z_of_argument regs rv = None ->
      Lea_failure regs r1 rv
-  | Lea_fail_p_E : forall p g b e a,
-     regs !! r1 = Some (inr ((p, g), b, e, a)) ->
+  | Lea_fail_p_E : forall p b e a,
+     regs !! r1 = Some (inr (p, b, e, a)) ->
      p = E ->
      Lea_failure regs r1 rv
   | Lea_fail_r1_noncap : forall n,
      regs !! r1 = Some (inl n) ->
      Lea_failure regs r1 rv
-  | Lea_fail_overflow : forall p g b e a z,
-     regs !! r1 = Some (inr ((p, g), b, e, a)) ->
+  | Lea_fail_overflow : forall p b e a z,
+     regs !! r1 = Some (inr (p, b, e, a)) ->
      z_of_argument regs rv = Some z ->
      (a + z)%a = None ->
      Lea_failure regs r1 rv
-  | Lea_fail_overflow_PC : forall p g b e a z a',
-     regs !! r1 = Some (inr ((p, g), b, e, a)) ->
+  | Lea_fail_overflow_PC : forall p b e a z a',
+     regs !! r1 = Some (inr (p, b, e, a)) ->
      z_of_argument regs rv = Some z ->
      (a + z)%a = Some a' ->
-     incrementPC (<[ r1 := inr ((p, g), b, e, a') ]> regs) = None ->
+     incrementPC (<[ r1 := inr (p, b, e, a') ]> regs) = None ->
      Lea_failure regs r1 rv
-  | Lea_fail_overflow_U : forall p g b e a z a',
-      regs !! r1 = Some (inr ((p, g), b, e, a)) ->
-      z_of_argument regs rv = Some z ->
-      (a + z)%a = Some a' ->
-      (match p with
-       | URW | URWL | URWX | URWLX => not (a' <= a)%a
-       | _ => False
-       end) ->
-      Lea_failure regs r1 rv
    .
 
   Inductive Lea_spec
     (regs: Reg) (r1: RegName) (rv: Z + RegName)
     (regs': Reg) : cap_lang.val → Prop
   :=
-  | Lea_spec_success : forall p g b e a z a',
-    regs !! r1 = Some (inr ((p, g), b, e, a)) ->
+  | Lea_spec_success : forall p b e a z a',
+    regs !! r1 = Some (inr (p, b, e, a)) ->
     p ≠ E ->
     z_of_argument regs rv = Some z ->
     (a + z)%a = Some a' ->
-    (match p with
-     | URW | URWL | URWX | URWLX => (a' <= a)%a
-     | _ => True
-     end) ->
     incrementPC
-      (<[ r1 := inr ((p, g), b, e, a') ]> regs) = Some regs' ->
+      (<[ r1 := inr (p, b, e, a') ]> regs) = Some regs' ->
     Lea_spec regs r1 rv regs' NextIV
 
   | Lea_spec_failure :
     Lea_failure regs r1 rv ->
     Lea_spec regs r1 rv regs' FailedV.
 
-   Lemma wp_lea Ep pc_p pc_g pc_b pc_e pc_a pc_p' r1 w arg (regs: Reg) :
+   Lemma wp_lea Ep pc_p pc_b pc_e pc_a r1 w arg (regs: Reg) :
      decodeInstrW w = Lea r1 arg →
-     PermFlows pc_p pc_p' →
-     isCorrectPC (inr ((pc_p, pc_g), pc_b, pc_e, pc_a)) →
-     regs !! PC = Some (inr ((pc_p, pc_g), pc_b, pc_e, pc_a)) →
+     isCorrectPC (inr (pc_p, pc_b, pc_e, pc_a)) →
+     regs !! PC = Some (inr (pc_p, pc_b, pc_e, pc_a)) →
      regs_of (Lea r1 arg) ⊆ dom _ regs →
-     {{{ ▷ pc_a ↦ₐ[pc_p'] w ∗
+     {{{ ▷ pc_a ↦ₐ w ∗
          ▷ [∗ map] k↦y ∈ regs, k ↦ᵣ y }}}
        Instr Executable @ Ep
      {{{ regs' retv, RET retv;
          ⌜ Lea_spec regs r1 arg regs' retv ⌝ ∗
-         pc_a ↦ₐ[pc_p'] w ∗
+         pc_a ↦ₐ w ∗
          [∗ map] k↦y ∈ regs', k ↦ᵣ y }}}.
    Proof.
-     iIntros (Hinstr Hfl Hvpc HPC Dregs φ) "(>Hpc_a & >Hmap) Hφ".
+     iIntros (Hinstr Hvpc HPC Dregs φ) "(>Hpc_a & >Hmap) Hφ".
      iApply wp_lift_atomic_head_step_no_fork; auto.
      iIntros (σ1 l1 l2 n) "Hσ1 /=". destruct σ1; simpl.
      iDestruct "Hσ1" as "[Hr Hm]".
-     assert (pc_p' ≠ O).
-     { destruct pc_p'; auto. destruct pc_p; inversion Hfl. inversion Hvpc; naive_solver. }
      iDestruct (gen_heap_valid_inclSepM with "Hr Hmap") as %Hregs.
      pose proof (regs_lookup_eq _ _ _ HPC) as HPC'.
      pose proof (lookup_weaken _ _ _ _ HPC Hregs).
-     iDestruct (@gen_heap_valid_cap with "Hm Hpc_a") as %Hpc_a; auto.
+     iDestruct (@gen_heap_valid with "Hm Hpc_a") as %Hpc_a; auto.
      iModIntro. iSplitR. by iPureIntro; apply normal_always_head_reducible.
      iNext. iIntros (e2 σ2 efs Hpstep).
      apply prim_step_exec_inv in Hpstep as (-> & -> & (c & -> & Hstep)).
@@ -105,7 +89,7 @@ Section cap_lang_rules.
      feed destruct (Hri r1) as [r1v [Hr'1 Hr1]]. by set_solver+.
      pose proof (regs_lookup_eq _ _ _ Hr1) as Hr1'.
      cbn in Hstep. rewrite Hr1' in Hstep.
-     destruct r1v as [| (([[p g] b] & e) & a) ] eqn:Hr1v.
+     destruct r1v as [| (([p b] & e) & a) ] eqn:Hr1v.
      { (* Failure: r1 is not a capability *)
        assert (c = Failed ∧ σ2 = (r, m)) as (-> & ->)
          by (destruct arg; inversion Hstep; auto).
@@ -145,23 +129,7 @@ Section cap_lang_rules.
            by (destruct p; inversion Hstep; auto).
          iFailWP "Hφ" Lea_fail_overflow. } }
 
-     assert (HU: match p with | URW | URWL | URWX | URWLX => not (a' <= a)%a | _ => False end \/ match p with | URW | URWL | URWX | URWLX => (a' <= a)%a | _ => True end) by (destruct (Addr_le_dec a' a); destruct p; auto).
-
-     destruct HU as [HU | HU].
-     { (* Failure: permission is uninitialized and try to increase reading bound *)
-       assert (c = Failed ∧ σ2 = (r, m)) as (-> & ->).
-       { unfold z_of_argument in Harg. destruct arg as [ z | r0 ].
-         - inversion Harg; subst z. rewrite Hoffset in Hstep.
-           destruct (Addr_le_dec a' a); destruct p; auto; try tauto; try congruence; inv Hstep; auto.
-         - destruct (Hri r0) as [r0v [Hr'0 Hr0]].
-           by unfold regs_of_argument; set_solver+.
-           rewrite /RegLocate Hr'0 Hr0 in Harg Hstep.
-           destruct r0v; [| congruence]. inversion Harg; subst z.
-           rewrite Hoffset in Hstep.
-           destruct (Addr_le_dec a' a); destruct p; auto; try tauto; try congruence; inv Hstep; auto. }
-       iFailWP "Hφ" Lea_fail_overflow_U. }
-
-     assert ((c, σ2) = updatePC (update_reg (r, m) r1 (inr (p, g, b, e, a')))) as HH.
+     assert ((c, σ2) = updatePC (update_reg (r, m) r1 (inr (p, b, e, a')))) as HH.
      { unfold z_of_argument in Harg. destruct arg as [ z | r0 ].
        { inversion Harg; subst z. rewrite Hoffset in Hstep.
          destruct p; auto; try congruence; destruct (Addr_le_dec a' a); try congruence; auto; solve_addr. }
@@ -173,10 +141,10 @@ Section cap_lang_rules.
          destruct p; auto; try congruence; destruct (Addr_le_dec a' a); try congruence; auto; solve_addr. } }
      clear Hstep. rewrite /update_reg /= in HH.
 
-     destruct (incrementPC (<[ r1 := inr ((p, g), b, e, a') ]> regs)) as [ regs' |] eqn:Hregs';
+     destruct (incrementPC (<[ r1 := inr (p, b, e, a') ]> regs)) as [ regs' |] eqn:Hregs';
        pose proof Hregs' as Hregs'2; cycle 1.
      { (* Failure: incrementing PC overflows *)
-       assert (incrementPC (<[ r1 := inr ((p, g, b, e, a'))]> r) = None).
+       assert (incrementPC (<[ r1 := inr ((p, b, e, a'))]> r) = None).
        { eapply incrementPC_overflow_mono; first eapply Hregs'.
          by rewrite lookup_insert_is_Some'; eauto.
          by apply insert_mono; eauto. }
@@ -187,7 +155,7 @@ Section cap_lang_rules.
      (* Success *)
 
      eapply (incrementPC_success_updatePC _ m) in Hregs'
-       as (p' & g' & b' & e' & a'' & a_pc' & HPC'' & Ha_pc' & HuPC & ->).
+       as (p' & g' & b' & e' & a'' & a_pc' & HPC'' & HuPC & ->).
      eapply updatePC_success_incl in HuPC. 2: by eapply insert_mono; eauto.
      rewrite HuPC in HH; clear HuPC; inversion HH; clear HH; subst c σ2. cbn.
      iFrame.
@@ -199,23 +167,23 @@ Section cap_lang_rules.
      Unshelve. all: assumption.
    Qed.
 
-   Lemma wp_lea_success_reg_PC Ep pc_p pc_g pc_b pc_e pc_a pc_a' w rv z a' pc_p' :
+   Lemma wp_lea_success_reg_PC Ep pc_p pc_b pc_e pc_a pc_a' w rv z a' :
      decodeInstrW w = Lea PC (inr rv) →
-     PermFlows pc_p pc_p' → isCorrectPC (inr ((pc_p,pc_g),pc_b,pc_e,pc_a)) →
+     isCorrectPC (inr (pc_p,pc_b,pc_e,pc_a)) →
      (a' + 1)%a = Some pc_a' →
      (pc_a + z)%a = Some a' →
      pc_p ≠ E →
 
-     {{{ ▷ PC ↦ᵣ inr ((pc_p,pc_g),pc_b,pc_e,pc_a)
-           ∗ ▷ pc_a ↦ₐ[pc_p'] w
+     {{{ ▷ PC ↦ᵣ inr (pc_p,pc_b,pc_e,pc_a)
+           ∗ ▷ pc_a ↦ₐ w
            ∗ ▷ rv ↦ᵣ inl z }}}
        Instr Executable @ Ep
        {{{ RET NextIV;
-           PC ↦ᵣ inr ((pc_p,pc_g),pc_b,pc_e,pc_a')
-              ∗ pc_a ↦ₐ[pc_p'] w
+           PC ↦ᵣ inr (pc_p,pc_b,pc_e,pc_a')
+              ∗ pc_a ↦ₐ w
               ∗ rv ↦ᵣ inl z }}}.
    Proof.
-     iIntros (Hinstr Hfl Hvpc Hpca' Ha' Hnep φ) "(>HPC & >Hpc_a & >Hrv) Hφ".
+     iIntros (Hinstr Hvpc Hpca' Ha' Hnep φ) "(>HPC & >Hpc_a & >Hrv) Hφ".
      iDestruct (map_of_regs_2 with "HPC Hrv") as "[Hmap %]".
      iApply (wp_lea with "[$Hmap Hpc_a]"); eauto; simplify_map_eq; eauto.
      by rewrite !dom_insert; set_solver+.
@@ -229,32 +197,28 @@ Section cap_lang_rules.
        iApply (regs_of_map_2 with "Hmap"); eauto. }
      { (* Failure (contradiction) *)
        destruct Hfail; try incrementPC_inv; simplify_map_eq; eauto. congruence.
-       inv Hvpc. naive_solver. }
+     }
    Qed.
 
-   Lemma wp_lea_success_reg Ep pc_p pc_g pc_b pc_e pc_a pc_a' w r1 rv p g b e a z a' pc_p' :
+   Lemma wp_lea_success_reg Ep pc_p pc_b pc_e pc_a pc_a' w r1 rv p b e a z a' :
      decodeInstrW w = Lea r1 (inr rv) →
-     PermFlows pc_p pc_p' → isCorrectPC (inr ((pc_p,pc_g),pc_b,pc_e,pc_a)) →
+     isCorrectPC (inr (pc_p,pc_b,pc_e,pc_a)) →
      (pc_a + 1)%a = Some pc_a' →
      (a + z)%a = Some a' →
-     r1 ≠ PC → p ≠ E →
-     (match p with
-      | URW | URWL | URWX | URWLX => (a' <= a)%a
-      | _ => True
-      end) ->
+     p ≠ E →
      
-     {{{ ▷ PC ↦ᵣ inr ((pc_p,pc_g),pc_b,pc_e,pc_a)
-           ∗ ▷ pc_a ↦ₐ[pc_p'] w
-           ∗ ▷ r1 ↦ᵣ inr ((p,g),b,e,a)
+     {{{ ▷ PC ↦ᵣ inr (pc_p,pc_b,pc_e,pc_a)
+           ∗ ▷ pc_a ↦ₐ w
+           ∗ ▷ r1 ↦ᵣ inr (p,b,e,a)
            ∗ ▷ rv ↦ᵣ inl z }}}
        Instr Executable @ Ep
        {{{ RET NextIV;
-           PC ↦ᵣ inr ((pc_p,pc_g),pc_b,pc_e,pc_a')
-              ∗ pc_a ↦ₐ[pc_p'] w
+           PC ↦ᵣ inr (pc_p,pc_b,pc_e,pc_a')
+              ∗ pc_a ↦ₐ w
               ∗ rv ↦ᵣ inl z
-              ∗ r1 ↦ᵣ inr ((p,g),b,e,a') }}}.
+              ∗ r1 ↦ᵣ inr (p,b,e,a') }}}.
    Proof.
-     iIntros (Hinstr Hfl Hvpc Hpca' Ha' Hne1 Hnep HU ϕ) "(>HPC & >Hpc_a & >Hr1 & >Hrv) Hφ".
+     iIntros (Hinstr Hvpc Hpca' Ha' Hnep ϕ) "(>HPC & >Hpc_a & >Hr1 & >Hrv) Hφ".
      iDestruct (map_of_regs_3 with "HPC Hrv Hr1") as "[Hmap (%&%&%)]".
      iApply (wp_lea with "[$Hmap Hpc_a]"); eauto; simplify_map_eq; eauto.
      by rewrite !dom_insert; set_solver+.
@@ -270,24 +234,24 @@ Section cap_lang_rules.
        iApply (regs_of_map_3 with "Hmap"); eauto. }
      { (* Failure (contradiction) *)
        destruct Hfail; try incrementPC_inv; simplify_map_eq; eauto. congruence.
-       destruct p0; tauto. }
+     }
    Qed.
 
-   Lemma wp_lea_success_z_PC Ep pc_p pc_g pc_b pc_e pc_a pc_a' w z a' pc_p' :
+   Lemma wp_lea_success_z_PC Ep pc_p pc_b pc_e pc_a pc_a' w z a' :
      decodeInstrW w = Lea PC (inl z) →
-     PermFlows pc_p pc_p' → isCorrectPC (inr ((pc_p,pc_g),pc_b,pc_e,pc_a)) →
+     isCorrectPC (inr (pc_p,pc_b,pc_e,pc_a)) →
      (a' + 1)%a = Some pc_a' →
      (pc_a + z)%a = Some a' →
      pc_p ≠ E →
 
-     {{{ ▷ PC ↦ᵣ inr ((pc_p,pc_g),pc_b,pc_e,pc_a)
-           ∗ ▷ pc_a ↦ₐ[pc_p'] w }}}
+     {{{ ▷ PC ↦ᵣ inr (pc_p,pc_b,pc_e,pc_a)
+           ∗ ▷ pc_a ↦ₐ w }}}
        Instr Executable @ Ep
      {{{ RET NextIV;
-         PC ↦ᵣ inr ((pc_p,pc_g),pc_b,pc_e,pc_a')
-            ∗ pc_a ↦ₐ[pc_p'] w }}}.
+         PC ↦ᵣ inr (pc_p,pc_b,pc_e,pc_a')
+            ∗ pc_a ↦ₐ w }}}.
    Proof.
-     iIntros (Hinstr Hfl Hvpc Hpca' Ha' Hnep ϕ) "(>HPC & >Hpc_a) Hφ".
+     iIntros (Hinstr Hvpc Hpca' Ha' Hnep ϕ) "(>HPC & >Hpc_a) Hφ".
      iDestruct (map_of_regs_1 with "HPC") as "Hmap".
      iApply (wp_lea with "[$Hmap Hpc_a]"); eauto; simplify_map_eq; eauto.
      by rewrite !dom_insert; set_solver+.
@@ -300,30 +264,26 @@ Section cap_lang_rules.
        rewrite !insert_insert. iApply (regs_of_map_1 with "Hmap"); eauto. }
      { (* Failure (contradiction) *)
        destruct Hfail; try incrementPC_inv; simplify_map_eq; eauto. congruence.
-       inv Hvpc. naive_solver. }
+     }
    Qed.
 
-   Lemma wp_lea_success_z Ep pc_p pc_g pc_b pc_e pc_a pc_a' w r1 p g b e a z a' pc_p' :
+   Lemma wp_lea_success_z Ep pc_p pc_b pc_e pc_a pc_a' w r1 p b e a z a' :
      decodeInstrW w = Lea r1 (inl z) →
-     PermFlows pc_p pc_p' → isCorrectPC (inr ((pc_p,pc_g),pc_b,pc_e,pc_a)) →
+     isCorrectPC (inr (pc_p,pc_b,pc_e,pc_a)) →
      (pc_a + 1)%a = Some pc_a' →
      (a + z)%a = Some a' →
-     r1 ≠ PC → p ≠ E →
-     (match p with
-      | URW | URWL | URWX | URWLX => (a' <= a)%a
-      | _ => True
-      end) ->
+     p ≠ E →
 
-     {{{ ▷ PC ↦ᵣ inr ((pc_p,pc_g),pc_b,pc_e,pc_a)
-           ∗ ▷ pc_a ↦ₐ[pc_p'] w
-           ∗ ▷ r1 ↦ᵣ inr ((p,g),b,e,a) }}}
+     {{{ ▷ PC ↦ᵣ inr (pc_p,pc_b,pc_e,pc_a)
+           ∗ ▷ pc_a ↦ₐ w
+           ∗ ▷ r1 ↦ᵣ inr (p,b,e,a) }}}
        Instr Executable @ Ep
      {{{ RET NextIV;
-         PC ↦ᵣ inr ((pc_p,pc_g),pc_b,pc_e,pc_a')
-            ∗ pc_a ↦ₐ[pc_p'] w
-            ∗ r1 ↦ᵣ inr ((p,g),b,e,a') }}}.
+         PC ↦ᵣ inr (pc_p,pc_b,pc_e,pc_a')
+            ∗ pc_a ↦ₐ w
+            ∗ r1 ↦ᵣ inr (p,b,e,a') }}}.
    Proof.
-     iIntros (Hinstr Hfl Hvpc Hpca' Ha' Hne1 Hnep HU ϕ) "(>HPC & >Hpc_a & >Hr1) Hφ".
+     iIntros (Hinstr Hvpc Hpca' Ha' Hnep ϕ) "(>HPC & >Hpc_a & >Hr1) Hφ".
      iDestruct (map_of_regs_2 with "HPC Hr1") as "[Hmap %]".
      iApply (wp_lea with "[$Hmap Hpc_a]"); eauto; simplify_map_eq; eauto.
      by rewrite !dom_insert; set_solver+.
@@ -338,7 +298,7 @@ Section cap_lang_rules.
        iDestruct (regs_of_map_2 with "Hmap") as "[? ?]"; eauto. iFrame. }
      { (* Failure (contradiction) *)
        destruct Hfail; try incrementPC_inv; simplify_map_eq; eauto. congruence.
-       destruct p0; tauto. }
+     }
    Qed.
 
 End cap_lang_rules.
