theories/rules/rules_Load.v
@@ -5,7 +5,7 @@ From iris.proofmode Require Import tactics.
 From iris.algebra Require Import frac.
 
 Section cap_lang_rules.
-  Context `{memG Σ, regG Σ, MonRef: MonRefG (leibnizO _) CapR_rtc Σ}.
+  Context `{memG Σ, regG Σ}.
   Context `{MachineParameters}.
   Implicit Types P Q : iProp Σ.
   Implicit Types σ : ExecConf.
@@ -17,33 +17,33 @@ Section cap_lang_rules.
   Implicit Types reg : gmap RegName Word.
   Implicit Types ms : gmap Addr Word.
 
-  Definition reg_allows_load (regs : Reg) (r : RegName) p g b e a  :=
-    regs !! r = Some (inr ((p, g), b, e, a)) ∧
-    readAllowed p = true ∧ withinBounds ((p, g), b, e, a) = true.
+  Definition reg_allows_load (regs : Reg) (r : RegName) p b e a  :=
+    regs !! r = Some (inr (p, b, e, a)) ∧
+    readAllowed p = true ∧ withinBounds (p, b, e, a) = true.
 
-  Inductive Load_failure (regs: Reg) (r1 r2: RegName) (mem : PermMem):=
+  Inductive Load_failure (regs: Reg) (r1 r2: RegName) (mem : gmap Addr Word) :=
   | Load_fail_const z:
       regs !! r2 = Some (inl z) ->
       Load_failure regs r1 r2 mem
-  | Load_fail_bounds p g b e a:
-      regs !! r2 = Some (inr ((p, g), b, e, a)) ->
-      (readAllowed p = false ∨ withinBounds ((p, g), b, e, a) = false) →
+  | Load_fail_bounds p b e a:
+      regs !! r2 = Some (inr (p, b, e, a)) ->
+      (readAllowed p = false ∨ withinBounds (p, b, e, a) = false) →
       Load_failure regs r1 r2 mem
   (* Notice how the None below also includes all cases where we read an inl value into the PC, because then incrementing it will fail *)
-  | Load_fail_invalid_PC p p' g b e a loadv:
-      regs !! r2 = Some (inr ((p, g), b, e, a)) ->
-      mem !! a = Some(p', loadv) →
+  | Load_fail_invalid_PC p b e a loadv:
+      regs !! r2 = Some (inr (p, b, e, a)) ->
+      mem !! a = Some loadv →
       incrementPC (<[ r1 := loadv ]> regs) = None ->
       Load_failure regs r1 r2 mem
   .
 
   Inductive Load_spec
     (regs: Reg) (r1 r2: RegName)
-    (regs': Reg) (mem : PermMem) : cap_lang.val → Prop
+    (regs': Reg) (mem : gmap Addr Word) : cap_lang.val → Prop
   :=
-  | Load_spec_success p p' g b e a loadv :
-    reg_allows_load regs r2 p g b e a →
-    mem !! a = Some(p', loadv) →
+  | Load_spec_success p b e a loadv :
+    reg_allows_load regs r2 p b e a →
+    mem !! a = Some loadv →
     incrementPC
       (<[ r1 := loadv ]> regs) = Some regs' ->
     Load_spec regs r1 r2 regs' mem NextIV
@@ -52,24 +52,24 @@ Section cap_lang_rules.
     Load_failure regs r1 r2 mem ->
     Load_spec regs r1 r2 regs' mem FailedV.
 
-  Definition allow_load_map_or_true r (regs : Reg) (mem : PermMem):=
-    ∃ p g b e a, read_reg_inr regs r p g b e a ∧
-      if decide (reg_allows_load regs r p g b e a) then
-        ∃ p' w, mem !! a = Some (p', w) ∧ p' ≠ O
+  Definition allow_load_map_or_true r (regs : Reg) (mem : gmap Addr Word):=
+    ∃ p b e a, read_reg_inr regs r p b e a ∧
+      if decide (reg_allows_load regs r p b e a) then
+        ∃ w, mem !! a = Some w 
       else True.
 
   Lemma allow_load_implies_loadv:
-    ∀ (r2 : RegName) (mem0 : PermMem) (r : Reg) (p : Perm) (g : Locality) (b e a : Addr),
+    ∀ (r2 : RegName) (mem0 : gmap Addr Word) (r : Reg) (p : Perm) (b e a : Addr),
       allow_load_map_or_true r2 r mem0
-      → r !r! r2 = inr (p, g, b, e, a)
+      → r !r! r2 = inr (p, b, e, a)
       → readAllowed p = true
-      → withinBounds (p, g, b, e, a) = true
-      → ∃ (p' : Perm) (loadv : Word),
-          mem0 !! a = Some (p', loadv) ∧ p' ≠ O.
+      → withinBounds (p, b, e, a) = true
+      → ∃ (loadv : Word),
+          mem0 !! a = Some loadv.
   Proof.
-    intros r2 mem0 r p g b e a HaLoad Hr2v Hra Hwb.
+    intros r2 mem0 r p b e a HaLoad Hr2v Hra Hwb.
     unfold allow_load_map_or_true in HaLoad.
-    destruct HaLoad as (?&?&?&?&?&[Hrr | Hrl]&Hmem).
+    destruct HaLoad as (?&?&?&?&[Hrr | Hrl]&Hmem).
     - assert (Hrr' := Hrr). option_locate_r_once r. rewrite Hrr2 in Hr2v; inversion Hr2v; subst.
       case_decide as HAL.
       * auto.
@@ -79,90 +79,82 @@ Section cap_lang_rules.
   Qed.
 
   Lemma mem_eq_implies_allow_load_map:
-    ∀ (regs : Reg)(mem : PermMem)(r2 : RegName) (w : Word) p g b e a
-      (p' : Perm)  ,
-      mem = <[a:=(p', w)]> ∅
-      → regs !! r2 = Some (inr (p,g,b,e,a))
-      → p' ≠ O
+    ∀ (regs : Reg)(mem : gmap Addr Word)(r2 : RegName) (w : Word) p b e a,
+      mem = <[a:=w]> ∅
+      → regs !! r2 = Some (inr (p,b,e,a))
       → allow_load_map_or_true r2 regs mem.
   Proof.
-    intros regs mem r2 w p g b e a p' Hmem Hrr2 Hpc_p'.
-    exists p,g,b,e,a; split.
+    intros regs mem r2 w p b e a Hmem Hrr2.
+    exists p,b,e,a; split.
     - left. by simplify_map_eq.
     - case_decide; last done.
-      exists p', w. simplify_map_eq. auto.
+      exists w. simplify_map_eq. auto.
   Qed.
 
   Lemma mem_neq_implies_allow_load_map:
-    ∀ (regs : Reg)(mem : PermMem)(r2 : RegName) (pc_a : Addr)
-      (w w' : Word) p g b e a
-      (pc_p' p' : Perm)  ,
+    ∀ (regs : Reg)(mem : gmap Addr Word)(r2 : RegName) (pc_a : Addr)
+      (w w' : Word) p b e a,
       a ≠ pc_a
-      → mem = <[pc_a:=(pc_p', w)]> (<[a:=(p', w')]> ∅)
-      → regs !! r2 = Some (inr (p,g,b,e,a))
-      → p' ≠ O
+      → mem = <[pc_a:=w]> (<[a:=w']> ∅)
+      → regs !! r2 = Some (inr (p,b,e,a))
       → allow_load_map_or_true r2 regs mem.
   Proof.
-    intros regs mem r2 pc_a w w' p g b e a pc_p' p' H4 Hrr2 Hp'.
-    exists p,g,b,e,a; split.
+    intros regs mem r2 pc_a w w' p b e a H4 Hrr2.
+    exists p,b,e,a; split.
     - left. by simplify_map_eq.
     - case_decide; last done.
-      exists p', w'. simplify_map_eq. split; auto.
+      exists w'. simplify_map_eq. split; auto.
   Qed.
 
   Lemma mem_implies_allow_load_map:
-    ∀ (regs : Reg)(mem : PermMem)(r2 : RegName) (pc_a : Addr)
-      (w w' : Word) p g b e a
-      (pc_p' p' : Perm)  ,
+    ∀ (regs : Reg)(mem : gmap Addr Word)(r2 : RegName) (pc_a : Addr)
+      (w w' : Word) p b e a,
       (if (a =? pc_a)%a
-       then mem = <[pc_a:=(pc_p', w)]> ∅
-       else mem = <[pc_a:=(pc_p', w)]> (<[a:=(p', w')]> ∅))
-      → regs !! r2 = Some (inr (p,g,b,e,a))
-      → (if (a =? pc_a)%a then True else p' ≠ O)
-      → pc_p' ≠ O
+       then mem = <[pc_a:=w]> ∅
+       else mem = <[pc_a:=w]> (<[a:=w']> ∅))
+      → regs !! r2 = Some (inr (p,b,e,a))
       → allow_load_map_or_true r2 regs mem.
   Proof.
-    intros regs mem r2 pc_a w w' p g b e a pc_p' p' H4 Hrr2 Hp' Hpc_p'.
+    intros regs mem r2 pc_a w w' p b e a H4 Hrr2.
     destruct (a =? pc_a)%a eqn:Heq.
       + apply Z.eqb_eq, z_of_eq in Heq. subst a. eapply mem_eq_implies_allow_load_map; eauto.
       + apply Z.eqb_neq in Heq.  eapply mem_neq_implies_allow_load_map; eauto. congruence.
   Qed.
 
   Lemma mem_implies_loadv:
-    ∀ (pc_a : Addr) (w w' : Word) (pc_p' p' p'0 : Perm) (a0 : Addr)
-      (mem0 : gmap Addr (Perm * Word)) (loadv : Word),
+    ∀ (pc_a : Addr) (w w' : Word) (a0 : Addr)
+      (mem0 : gmap Addr Word) (loadv : Word),
       (if (a0 =? pc_a)%a
-       then mem0 = <[pc_a:=(pc_p', w)]> ∅
-       else mem0 = <[pc_a:=(pc_p', w)]> (<[a0:=(p', w')]> ∅))→
-      mem0 !! a0 = Some (p'0, loadv) →
+       then mem0 = <[pc_a:=w]> ∅
+       else mem0 = <[pc_a:=w]> (<[a0:=w']> ∅))→
+      mem0 !! a0 = Some loadv →
       loadv = (if (a0 =? pc_a)%a then w else w').
   Proof.
-    intros pc_a w w' pc_p' p' p'0  a0 mem0 loadv H4 H6.
+    intros pc_a w w' a0 mem0 loadv H4 H6.
     destruct (a0 =? pc_a)%a eqn:Heq; rewrite H4 in H6.
     + apply Z.eqb_eq, z_of_eq in Heq; subst a0. by simplify_map_eq.
     + apply Z.eqb_neq in Heq. rewrite lookup_insert_ne in H6; last congruence. by simplify_map_eq.
   Qed.
 
    Lemma wp_load Ep
-     pc_p pc_g pc_b pc_e pc_a pc_p'
+     pc_p pc_b pc_e pc_a
      r1 r2 w mem regs :
    decodeInstrW w = Load r1 r2 →
-   pc_p' ≠ O →
-   isCorrectPC (inr ((pc_p, pc_g), pc_b, pc_e, pc_a)) →
-   regs !! PC = Some (inr ((pc_p, pc_g), pc_b, pc_e, pc_a)) →
+   isCorrectPC (inr (pc_p, pc_b, pc_e, pc_a)) →
+   regs !! PC = Some (inr (pc_p, pc_b, pc_e, pc_a)) →
    regs_of (Load r1 r2) ⊆ dom _ regs →
-   mem !! pc_a = Some (pc_p', w) →
+   mem !! pc_a = Some w →
    allow_load_map_or_true r2 regs mem →
 
-   {{{ (▷ [∗ map] a↦pw ∈ mem, ∃ p w, ⌜pw = (p,w)⌝ ∗ a ↦ₐ[p] w) ∗
+   {{{ (▷ [∗ map] a↦w ∈ mem, a ↦ₐ w) ∗
        ▷ [∗ map] k↦y ∈ regs, k ↦ᵣ y }}}
      Instr Executable @ Ep
    {{{ regs' retv, RET retv;
        ⌜ Load_spec regs r1 r2 regs' mem retv⌝ ∗
-         ([∗ map] a↦pw ∈ mem, ∃ p w, ⌜pw = (p,w)⌝ ∗ a ↦ₐ[p] w) ∗
+         ([∗ map] a↦w ∈ mem, a ↦ₐ w) ∗
          [∗ map] k↦y ∈ regs', k ↦ᵣ y }}}.
    Proof.
-     iIntros (Hinstr Hfl Hvpc HPC Dregs Hmem_pc HaLoad φ) "(>Hmem & >Hmap) Hφ".
+     iIntros (Hinstr Hvpc HPC Dregs Hmem_pc HaLoad φ) "(>Hmem & >Hmap) Hφ".
      iApply wp_lift_atomic_head_step_no_fork; auto.
      iIntros (σ1 l1 l2 n) "[Hr Hm] /=". destruct σ1; simpl.
      iDestruct (gen_heap_valid_inclSepM with "Hr Hmap") as %Hregs.
@@ -175,7 +167,7 @@ Section cap_lang_rules.
      pose proof (regs_lookup_eq _ _ _ Hr'1) as Hr''1.
      pose proof (regs_lookup_eq _ _ _ Hr'2) as Hr''2.
      (* Derive the PC in memory *)
-     iDestruct (gen_mem_valid_inSepM pc_a _ _ _ _ mem _ m with "Hm Hmem") as %Hma; eauto.
+     iDestruct (gen_mem_valid_inSepM pc_a _ _ _ mem _ m with "Hm Hmem") as %Hma; eauto.
 
      iModIntro.
      iSplitR. by iPureIntro; apply normal_always_head_reducible.
@@ -187,13 +179,13 @@ Section cap_lang_rules.
      cbn in Hstep. rewrite Hrr2 in Hstep.
 
      (* Now we start splitting on the different cases in the Load spec, and prove them one at a time *)
-     destruct r2v as  [| (([[p g] b] & e) & a) ] eqn:Hr2v.
+     destruct r2v as  [| (([p b] & e) & a) ] eqn:Hr2v.
      { (* Failure: r2 is not a capability *)
        symmetry in Hstep; inversion Hstep; clear Hstep. subst c σ2.
         iFailWP "Hφ" Load_fail_const.
      }
 
-     destruct (readAllowed p && withinBounds ((p, g), b, e, a)) eqn:HRA; rewrite HRA in Hstep.
+     destruct (readAllowed p && withinBounds (p, b, e, a)) eqn:HRA; rewrite HRA in Hstep.
      2 : { (* Failure: r2 is either not within bounds or doesnt allow reading *)
        symmetry in Hstep; inversion Hstep; clear Hstep. subst c σ2.
        apply andb_false_iff in HRA.
@@ -202,9 +194,9 @@ Section cap_lang_rules.
      apply andb_true_iff in HRA; destruct HRA as (Hra & Hwb).
 
      (* Prove that a is in the memory map now, otherwise we cannot continue *)
-     pose proof (allow_load_implies_loadv r2 mem regs p g b e a) as (p' & loadv & Hmema & HPFp); auto.
+     pose proof (allow_load_implies_loadv r2 mem regs p b e a) as (loadv & Hmema); auto.
 
-     iDestruct (mem_v_implies_m_v mem m p g b e a p' loadv with "Hmem Hm" ) as %Hma ; auto.
+     iDestruct (mem_v_implies_m_v mem m b e a loadv with "Hmem Hm" ) as %Hma ; auto.
 
      rewrite Hma in Hstep.
      destruct (incrementPC (<[ r1 := loadv ]> regs)) as  [ regs' |] eqn:Hregs'.
@@ -224,7 +216,7 @@ Section cap_lang_rules.
      (* Success *)
      rewrite /update_reg /= in Hstep.
      eapply (incrementPC_success_updatePC _ m) in Hregs'
-       as (p1 & g1 & b1 & e1 & a1 & a_pc1 & HPC'' & Ha_pc' & HuPC & ->).
+       as (p1 & b1 & e1 & a1 & a_pc1 & HPC'' & Ha_pc' & HuPC & ->).
      eapply updatePC_success_incl in HuPC. 2: by eapply insert_mono.
      rewrite HuPC in Hstep; clear HuPC; inversion Hstep; clear Hstep; subst c σ2. cbn.
      iFrame.
@@ -240,40 +232,30 @@ Section cap_lang_rules.
      Unshelve. all: auto.
    Qed.
 
-  Lemma wp_load_success E r1 r2 pc_p pc_g pc_b pc_e pc_a w w' w'' p g b e a pc_a'
-        pc_p' p' :
+  Lemma wp_load_success E r1 r2 pc_p pc_b pc_e pc_a w w' w'' p b e a pc_a' :
     decodeInstrW w = Load r1 r2 →
-    PermFlows pc_p pc_p' →
-    isCorrectPC (inr ((pc_p,pc_g),pc_b,pc_e,pc_a)) →
-    readAllowed p = true ∧ withinBounds ((p, g), b, e, a) = true →
+    isCorrectPC (inr (pc_p,pc_b,pc_e,pc_a)) →
+    readAllowed p = true ∧ withinBounds (p, b, e, a) = true →
     (pc_a + 1)%a = Some pc_a' →
 
-    {{{ ▷ PC ↦ᵣ inr ((pc_p,pc_g),pc_b,pc_e,pc_a)
-          ∗ ▷ pc_a ↦ₐ[pc_p'] w
+    {{{ ▷ PC ↦ᵣ inr (pc_p,pc_b,pc_e,pc_a)
+          ∗ ▷ pc_a ↦ₐ w
           ∗ ▷ r1 ↦ᵣ w''  
-          ∗ ▷ r2 ↦ᵣ inr ((p,g),b,e,a)
-          ∗ (if (eqb_addr a pc_a) then emp else ⌜PermFlows p p'⌝ ∗ ▷ a ↦ₐ[p'] w') }}}
+          ∗ ▷ r2 ↦ᵣ inr (p,b,e,a)
+          ∗ (if (eqb_addr a pc_a) then emp else ▷ a ↦ₐ w') }}}
       Instr Executable @ E
       {{{ RET NextIV;
-          PC ↦ᵣ inr ((pc_p,pc_g),pc_b,pc_e,pc_a')
+          PC ↦ᵣ inr (pc_p,pc_b,pc_e,pc_a')
              ∗ r1 ↦ᵣ (if (eqb_addr a pc_a) then w else w')
-             ∗ pc_a ↦ₐ[pc_p'] w
-             ∗ r2 ↦ᵣ inr ((p,g),b,e,a)
-             ∗ (if (eqb_addr a pc_a) then emp else a ↦ₐ[p'] w') }}}. 
+             ∗ pc_a ↦ₐ w
+             ∗ r2 ↦ᵣ inr (p,b,e,a)
+             ∗ (if (eqb_addr a pc_a) then emp else a ↦ₐ w') }}}. 
   Proof.
-    iIntros (Hinstr Hfl Hvpc [Hra Hwb] Hpca' φ)
+    iIntros (Hinstr Hvpc [Hra Hwb] Hpca' φ)
             "(>HPC & >Hi & >Hr1 & >Hr2 & Hr2a) Hφ".
     iDestruct (map_of_regs_3 with "HPC Hr1 Hr2") as "[Hmap (%&%&%)]".
-    iDestruct (extract_sep_if_split with "Hr2a") as "[Hfl' Hr2a]".
     iDestruct (memMap_resource_2gen_clater with "Hi Hr2a") as (mem) "[>Hmem Hmem']".
     iDestruct "Hmem'" as %Hmem.
-    pose proof (correctPC_nonO _ _ _ _ _ _ Hfl Hvpc) as Hpc_p'.
-    iAssert (⌜if (a =? pc_a)%a then True else p' ≠ O⌝)%I with "[Hfl']" as %Hp'.
-    {
-      destruct (a =? pc_a)%a; first by auto.
-      iDestruct "Hfl'" as %Hfl'.
-      iPureIntro. apply (readAllowed_nonO _ _ Hfl' Hra).
-    }
 
     iApply (wp_load with "[$Hmap $Hmem]"); eauto; simplify_map_eq; eauto.
     { by rewrite !dom_insert; set_solver+. }
@@ -289,7 +271,7 @@ Section cap_lang_rules.
        iDestruct (memMap_resource_2gen_d with "[Hmem]") as "[Hpc_a Ha]".
        {iExists mem; iSplitL; auto. }
        incrementPC_inv.
-       pose proof (mem_implies_loadv _ _ _ _ _ _ _ _ _ Hmem H6) as Hloadv; eauto.
+       pose proof (mem_implies_loadv _ _ _ _ _ _ Hmem H6) as Hloadv; eauto.
        simplify_map_eq.
        rewrite (insert_commute _ PC r1) // insert_insert (insert_commute _ r1 PC) // insert_insert.
        iDestruct (regs_of_map_3 with "[$Hmap]") as "[HPC [Hr1 Hr2] ]"; eauto.
@@ -299,38 +281,28 @@ Section cap_lang_rules.
        destruct o. all: congruence. }
   Qed.
 
-  Lemma wp_load_success_same E r1 pc_p pc_g pc_b pc_e pc_a w w' w'' p g b e a pc_a'
-        pc_p' p' :
+  Lemma wp_load_success_same E r1 pc_p pc_b pc_e pc_a w w' w'' p b e a pc_a' :
     decodeInstrW w = Load r1 r1 →
-    PermFlows pc_p pc_p' →
-    isCorrectPC (inr ((pc_p,pc_g),pc_b,pc_e,pc_a)) →
-    readAllowed p = true ∧ withinBounds ((p, g), b, e, a) = true →
+    isCorrectPC (inr (pc_p,pc_b,pc_e,pc_a)) →
+    readAllowed p = true ∧ withinBounds (p, b, e, a) = true →
     (pc_a + 1)%a = Some pc_a' →
 
-    {{{ ▷ PC ↦ᵣ inr ((pc_p,pc_g),pc_b,pc_e,pc_a)
-          ∗ ▷ pc_a ↦ₐ[pc_p'] w
-          ∗ ▷ r1 ↦ᵣ inr ((p,g),b,e,a)
-          ∗ (if (a =? pc_a)%a then emp else ⌜PermFlows p p'⌝ ∗ ▷ a ↦ₐ[p'] w') }}}
+    {{{ ▷ PC ↦ᵣ inr (pc_p,pc_b,pc_e,pc_a)
+          ∗ ▷ pc_a ↦ₐ w
+          ∗ ▷ r1 ↦ᵣ inr (p,b,e,a)
+          ∗ (if (a =? pc_a)%a then emp else ▷ a ↦ₐ w') }}}
       Instr Executable @ E
       {{{ RET NextIV;
-          PC ↦ᵣ inr ((pc_p,pc_g),pc_b,pc_e,pc_a')
+          PC ↦ᵣ inr (pc_p,pc_b,pc_e,pc_a')
              ∗ r1 ↦ᵣ (if (a =? pc_a)%a then w else w')
-             ∗ pc_a ↦ₐ[pc_p'] w
-             ∗ (if (a =? pc_a)%a then emp else a ↦ₐ[p'] w') }}}. 
+             ∗ pc_a ↦ₐ w
+             ∗ (if (a =? pc_a)%a then emp else a ↦ₐ w') }}}. 
   Proof.
-    iIntros (Hinstr Hfl Hvpc [Hra Hwb] Hpca' φ)
+    iIntros (Hinstr Hvpc [Hra Hwb] Hpca' φ)
             "(>HPC & >Hi & >Hr1 & Hr1a) Hφ".
     iDestruct (map_of_regs_2 with "HPC Hr1") as "[Hmap %]".
-    iDestruct (extract_sep_if_split with "Hr1a") as "[Hfl' Hr1a]".
     iDestruct (memMap_resource_2gen_clater with "Hi Hr1a") as (mem) "[>Hmem Hmem']".
     iDestruct "Hmem'" as %Hmem.
-    pose proof (correctPC_nonO _ _ _ _ _ _ Hfl Hvpc) as Hpc_p'.
-    iAssert (⌜if (a =? pc_a)%a then True else p' ≠ O⌝)%I with "[Hfl']" as %Hp'.
-    {
-      destruct (a =? pc_a)%a; first by auto.
-      iDestruct "Hfl'" as %Hfl'.
-      iPureIntro. apply (readAllowed_nonO _ _ Hfl' Hra).
-    }
 
     iApply (wp_load with "[$Hmap $Hmem]"); eauto; simplify_map_eq; eauto.
     { by rewrite !dom_insert; set_solver+. }
@@ -346,7 +318,7 @@ Section cap_lang_rules.
        iDestruct (memMap_resource_2gen_d with "[Hmem]") as "[Hpc_a Ha]".
        {iExists mem; iSplitL; auto. }
        incrementPC_inv.
-       pose proof (mem_implies_loadv _ _ _ _ _ _ _ _ _ Hmem H4) as Hloadv; eauto.
+       pose proof (mem_implies_loadv _ _ _ _ _ _ Hmem H4) as Hloadv; eauto.
        simplify_map_eq.
        rewrite (insert_commute _ PC r1) // insert_insert (insert_commute _ r1 PC) // insert_insert.
        iDestruct (regs_of_map_2 with "[$Hmap]") as "[HPC Hr1]"; eauto. iFrame. }
@@ -356,35 +328,31 @@ Section cap_lang_rules.
     Qed.
 
   (* If a points to a capability, the load into PC success if its address can be incr *)
-  Lemma wp_load_success_PC E r2 pc_p pc_g pc_b pc_e pc_a w
-        p g b e a p' g' b' e' a' a'' pc_p' p'' :
+  Lemma wp_load_success_PC E r2 pc_p pc_b pc_e pc_a w
+        p b e a p' b' e' a' a'' :
     decodeInstrW w = Load PC r2 →
-    PermFlows pc_p pc_p' →
-    PermFlows p p'' →
-    isCorrectPC (inr ((pc_p,pc_g),pc_b,pc_e,pc_a)) →
-    readAllowed p = true ∧ withinBounds ((p, g), b, e, a) = true →
+    isCorrectPC (inr (pc_p,pc_b,pc_e,pc_a)) →
+    readAllowed p = true ∧ withinBounds (p, b, e, a) = true →
     (a' + 1)%a = Some a'' →
 
-    {{{ ▷ PC ↦ᵣ inr ((pc_p,pc_g),pc_b,pc_e,pc_a)
-          ∗ ▷ pc_a ↦ₐ[pc_p'] w
-          ∗ ▷ r2 ↦ᵣ inr ((p,g),b,e,a)
-          ∗ ▷ a ↦ₐ[p''] inr ((p',g'),b',e',a') }}} 
+    {{{ ▷ PC ↦ᵣ inr (pc_p,pc_b,pc_e,pc_a)
+          ∗ ▷ pc_a ↦ₐ w
+          ∗ ▷ r2 ↦ᵣ inr (p,b,e,a)
+          ∗ ▷ a ↦ₐ inr (p',b',e',a') }}} 
       Instr Executable @ E
       {{{ RET NextIV;
-          PC ↦ᵣ inr ((p',g'),b',e',a'')
-             ∗ pc_a ↦ₐ[pc_p'] w
-             ∗ r2 ↦ᵣ inr ((p,g),b,e,a)
-             ∗ a ↦ₐ[p''] inr ((p',g'),b',e',a') }}}. 
+          PC ↦ᵣ inr (p',b',e',a'')
+             ∗ pc_a ↦ₐ w
+             ∗ r2 ↦ᵣ inr (p,b,e,a)
+             ∗ a ↦ₐ inr (p',b',e',a') }}}. 
   Proof.
-    iIntros (Hinstr Hfl Hfl' Hvpc [Hra Hwb] Hpca' φ)
+    iIntros (Hinstr Hvpc [Hra Hwb] Hpca' φ)
             "(>HPC & >Hi & >Hr2 & >Hr2a) Hφ".
-    pose proof (readAllowed_nonO _ _ Hfl' Hra) as Hp''.
-    pose proof (correctPC_nonO _ _ _ _ _ _ Hfl Hvpc) as Hpc_p'.
     iDestruct (map_of_regs_2 with "HPC Hr2") as "[Hmap %]".
     iDestruct (memMap_resource_2ne_apply with "Hi Hr2a") as "[Hmem %]"; auto.
     iApply (wp_load with "[$Hmap $Hmem]"); eauto; simplify_map_eq; eauto.
     { by rewrite !dom_insert; set_solver+. }
-    { eapply mem_neq_implies_allow_load_map with (a := a) (p' := p'')(pc_a := pc_a); eauto.
+    { eapply mem_neq_implies_allow_load_map with (a := a) (pc_a := pc_a); eauto.
       by simplify_map_eq. }
     iNext. iIntros (regs' retv) "(#Hspec & Hmem & Hmap)".
     iDestruct "Hspec" as %Hspec.
@@ -403,23 +371,22 @@ Section cap_lang_rules.
        destruct o. all: congruence. }
   Qed.
 
-  Lemma wp_load_success_fromPC E r1 pc_p pc_g pc_b pc_e pc_a pc_a' w w'' pc_p' :
+  Lemma wp_load_success_fromPC E r1 pc_p pc_b pc_e pc_a pc_a' w w'' :
     decodeInstrW w = Load r1 PC →
-    PermFlows pc_p pc_p' → isCorrectPC (inr ((pc_p,pc_g),pc_b,pc_e,pc_a)) →
+    isCorrectPC (inr (pc_p,pc_b,pc_e,pc_a)) →
     (pc_a + 1)%a = Some pc_a' →
 
-    {{{ ▷ PC ↦ᵣ inr ((pc_p,pc_g),pc_b,pc_e,pc_a)
-          ∗ ▷ pc_a ↦ₐ[pc_p'] w
+    {{{ ▷ PC ↦ᵣ inr (pc_p,pc_b,pc_e,pc_a)
+          ∗ ▷ pc_a ↦ₐ w
           ∗ ▷ r1 ↦ᵣ w'' }}} 
       Instr Executable @ E
       {{{ RET NextIV;
-          PC ↦ᵣ inr ((pc_p,pc_g),pc_b,pc_e,pc_a')
-             ∗ pc_a ↦ₐ[pc_p'] w
+          PC ↦ᵣ inr (pc_p,pc_b,pc_e,pc_a')
+             ∗ pc_a ↦ₐ w
              ∗ r1 ↦ᵣ w }}}. 
   Proof.
-    iIntros (Hinstr Hfl Hvpc Hpca' φ)
+    iIntros (Hinstr Hvpc Hpca' φ)
             "(>HPC & >Hi & >Hr1) Hφ".
-    pose proof (correctPC_nonO _ _ _ _ _ _ Hfl Hvpc) as Hpc_p'.
     iDestruct (map_of_regs_2 with "HPC Hr1") as "[Hmap %]".
     rewrite memMap_resource_1.
     iApply (wp_load with "[$Hmap $Hi]"); eauto; simplify_map_eq; eauto.
