theories/rules/rules_Mov.v
@@ -5,7 +5,7 @@ From iris.proofmode Require Import tactics.
 From iris.algebra Require Import frac.
 
 Section cap_lang_rules.
-  Context `{memG Σ, regG Σ, MonRef: MonRefG (leibnizO _) CapR_rtc Σ}.
+  Context `{memG Σ, regG Σ}.
   Context `{MachineParameters}.
   Implicit Types P Q : iProp Σ.
   Implicit Types σ : ExecConf.
@@ -27,31 +27,27 @@ Section cap_lang_rules.
       incrementPC (<[ dst := w ]> regs) = None →
       Mov_spec regs dst src regs' FailedV.
 
-  Lemma wp_Mov Ep pc_p pc_g pc_b pc_e pc_a pc_p' w dst src regs :
+  Lemma wp_Mov Ep pc_p pc_b pc_e pc_a  w dst src regs :
     decodeInstrW w = Mov dst src ->
-    PermFlows pc_p pc_p' →
-    isCorrectPC (inr ((pc_p, pc_g), pc_b, pc_e, pc_a)) →
-    regs !! PC = Some (inr ((pc_p, pc_g), pc_b, pc_e, pc_a)) →
+    isCorrectPC (inr (pc_p, pc_b, pc_e, pc_a)) →
+    regs !! PC = Some (inr (pc_p, pc_b, pc_e, pc_a)) →
     regs_of (Mov dst src) ⊆ dom _ regs →
-    {{{ ▷ pc_a ↦ₐ[pc_p'] w ∗
+    {{{ ▷ pc_a ↦ₐ w ∗
         ▷ [∗ map] k↦y ∈ regs, k ↦ᵣ y }}}
       Instr Executable @ Ep
     {{{ regs' retv, RET retv;
         ⌜ Mov_spec regs dst src regs' retv ⌝ ∗
-        pc_a ↦ₐ[pc_p'] w ∗
+        pc_a ↦ₐ w ∗
         [∗ map] k↦y ∈ regs', k ↦ᵣ y }}}.
   Proof.
-    iIntros (Hinstr Hfl Hvpc HPC Dregs φ) "(>Hpc_a & >Hmap) Hφ".
+    iIntros (Hinstr Hvpc HPC Dregs φ) "(>Hpc_a & >Hmap) Hφ".
     iApply wp_lift_atomic_head_step_no_fork; auto.
     iIntros (σ1 l1 l2 n) "Hσ1 /=". destruct σ1; simpl.
     iDestruct "Hσ1" as "[Hr Hm]".
-    assert (pc_p' ≠ O).
-    { destruct pc_p'; auto. destruct pc_p; inversion Hfl.
-      inversion Hvpc; naive_solver. }
     iDestruct (gen_heap_valid_inclSepM with "Hr Hmap") as %Hregs.
     have HPC' := regs_lookup_eq _ _ _ HPC.
     have ? := lookup_weaken _ _ _ _ HPC Hregs.
-    iDestruct (@gen_heap_valid_cap with "Hm Hpc_a") as %Hpc_a; auto.
+    iDestruct (@gen_heap_valid with "Hm Hpc_a") as %Hpc_a; auto.
     iModIntro. iSplitR. by iPureIntro; apply normal_always_head_reducible.
     iNext. iIntros (e2 σ2 efs Hpstep).
     apply prim_step_exec_inv in Hpstep as (-> & -> & (c & -> & Hstep)).
@@ -82,7 +78,7 @@ Section cap_lang_rules.
       iFrame. iApply "Hφ"; iFrame. iPureIntro. econstructor; eauto. }
 
     eapply (incrementPC_success_updatePC _ m) in Hregs'
-      as (p' & g' & b' & e' & a'' & a_pc' & HPC'' & Ha_pc' & HuPC & ->).
+      as (p' & g' & b' & e' & a'' & a_pc' & HPC'' & HuPC & ->).
     eapply updatePC_success_incl with (m':=m) in HuPC. 2: by eapply insert_mono; eauto.
     simplify_pair_eq. iFrame.
     iMod ((gen_heap_update_inSepM _ _ dst) with "Hr Hmap") as "[Hr Hmap]"; eauto.
@@ -90,23 +86,21 @@ Section cap_lang_rules.
     iFrame. iModIntro. iApply "Hφ". iFrame. iPureIntro. econstructor; eauto.
   Qed.
 
-  Lemma wp_move_success_z E pc_p pc_g pc_b pc_e pc_a pc_a' w r1 wr1 z pc_p' :
+  Lemma wp_move_success_z E pc_p pc_b pc_e pc_a pc_a' w r1 wr1 z :
     decodeInstrW w = Mov r1 (inl z) →
-    PermFlows pc_p pc_p' →
-    isCorrectPC (inr ((pc_p,pc_g),pc_b,pc_e,pc_a)) →
+    isCorrectPC (inr (pc_p,pc_b,pc_e,pc_a)) →
     (pc_a + 1)%a = Some pc_a' →
-    PC ≠ r1 →
 
-    {{{ ▷ PC ↦ᵣ inr ((pc_p,pc_g),pc_b,pc_e,pc_a)
-        ∗ ▷ pc_a ↦ₐ[pc_p'] w
+    {{{ ▷ PC ↦ᵣ inr (pc_p,pc_b,pc_e,pc_a)
+        ∗ ▷ pc_a ↦ₐ w
         ∗ ▷ r1 ↦ᵣ wr1 }}}
       Instr Executable @ E
       {{{ RET NextIV;
-          PC ↦ᵣ inr ((pc_p,pc_g),pc_b,pc_e,pc_a')
-          ∗ pc_a ↦ₐ[pc_p'] w
+          PC ↦ᵣ inr (pc_p,pc_b,pc_e,pc_a')
+          ∗ pc_a ↦ₐ w
           ∗ r1 ↦ᵣ inl z }}}.
   Proof.
-    iIntros (Hinstr Hfl Hvpc Hpca' Hne ϕ) "(>HPC & >Hpc_a & >Hr1) Hφ".
+    iIntros (Hinstr Hvpc Hpca' ϕ) "(>HPC & >Hpc_a & >Hr1) Hφ".
     iDestruct (map_of_regs_2 with "HPC Hr1") as "[Hmap %]".
     iApply (wp_Mov with "[$Hmap Hpc_a]"); eauto; simplify_map_eq; eauto.
     by unfold regs_of; rewrite !dom_insert; set_solver+.
@@ -121,25 +115,23 @@ Section cap_lang_rules.
       incrementPC_inv; simplify_map_eq; eauto. congruence. }
   Qed.
 
-  Lemma wp_move_success_reg E pc_p pc_g pc_b pc_e pc_a pc_a' w r1 wr1 rv wrv pc_p' :
+  Lemma wp_move_success_reg E pc_p pc_b pc_e pc_a pc_a' w r1 wr1 rv wrv :
     decodeInstrW w = Mov r1 (inr rv) →
-    PermFlows pc_p pc_p' →
-    isCorrectPC (inr ((pc_p,pc_g),pc_b,pc_e,pc_a)) →
+    isCorrectPC (inr (pc_p,pc_b,pc_e,pc_a)) →
     (pc_a + 1)%a = Some pc_a' →
-    PC ≠ r1 →
 
-    {{{ ▷ PC ↦ᵣ inr ((pc_p,pc_g),pc_b,pc_e,pc_a)
-        ∗ ▷ pc_a ↦ₐ[pc_p'] w
+    {{{ ▷ PC ↦ᵣ inr (pc_p,pc_b,pc_e,pc_a)
+        ∗ ▷ pc_a ↦ₐ w
         ∗ ▷ r1 ↦ᵣ wr1
         ∗ ▷ rv ↦ᵣ wrv }}}
       Instr Executable @ E
       {{{ RET NextIV;
-          PC ↦ᵣ inr ((pc_p,pc_g),pc_b,pc_e,pc_a')
-          ∗ pc_a ↦ₐ[pc_p'] w
+          PC ↦ᵣ inr (pc_p,pc_b,pc_e,pc_a')
+          ∗ pc_a ↦ₐ w
           ∗ r1 ↦ᵣ wrv
           ∗ rv ↦ᵣ wrv }}}.
   Proof.
-    iIntros (Hinstr Hfl Hvpc Hpca' Hne ϕ) "(>HPC & >Hpc_a & >Hr1 & >Hrv) Hφ".
+    iIntros (Hinstr Hvpc Hpca' ϕ) "(>HPC & >Hpc_a & >Hr1 & >Hrv) Hφ".
     iDestruct (map_of_regs_3 with "HPC Hr1 Hrv") as "[Hmap (%&%&%)]".
     iApply (wp_Mov with "[$Hmap Hpc_a]"); eauto; simplify_map_eq; eauto.
     by unfold regs_of; rewrite !dom_insert; set_solver+.
@@ -154,23 +146,21 @@ Section cap_lang_rules.
       incrementPC_inv; simplify_map_eq; eauto. congruence. }
   Qed.
 
-  Lemma wp_move_success_reg_same E pc_p pc_g pc_b pc_e pc_a pc_a' w r1 wr1 pc_p' :
+  Lemma wp_move_success_reg_same E pc_p pc_b pc_e pc_a pc_a' w r1 wr1 :
     decodeInstrW w = Mov r1 (inr r1) →
-    PermFlows pc_p pc_p' →
-    isCorrectPC (inr ((pc_p,pc_g),pc_b,pc_e,pc_a)) →
+    isCorrectPC (inr (pc_p,pc_b,pc_e,pc_a)) →
     (pc_a + 1)%a = Some pc_a' →
-    PC ≠ r1 →
 
-    {{{ ▷ PC ↦ᵣ inr ((pc_p,pc_g),pc_b,pc_e,pc_a)
-        ∗ ▷ pc_a ↦ₐ[pc_p'] w
+    {{{ ▷ PC ↦ᵣ inr (pc_p,pc_b,pc_e,pc_a)
+        ∗ ▷ pc_a ↦ₐ w
         ∗ ▷ r1 ↦ᵣ wr1 }}}
       Instr Executable @ E
       {{{ RET NextIV;
-          PC ↦ᵣ inr ((pc_p,pc_g),pc_b,pc_e,pc_a')
-          ∗ pc_a ↦ₐ[pc_p'] w
+          PC ↦ᵣ inr (pc_p,pc_b,pc_e,pc_a')
+          ∗ pc_a ↦ₐ w
           ∗ r1 ↦ᵣ wr1 }}}.
   Proof.
-    iIntros (Hinstr Hfl Hvpc Hpca' Hne ϕ) "(>HPC & >Hpc_a & >Hr1) Hφ".
+    iIntros (Hinstr Hvpc Hpca' ϕ) "(>HPC & >Hpc_a & >Hr1) Hφ".
     iDestruct (map_of_regs_2 with "HPC Hr1") as "[Hmap %]".
     iApply (wp_Mov with "[$Hmap Hpc_a]"); eauto; simplify_map_eq; eauto.
     by unfold regs_of; rewrite !dom_insert; set_solver+.
@@ -185,20 +175,19 @@ Section cap_lang_rules.
       incrementPC_inv; simplify_map_eq; eauto. congruence. }
   Qed.
 
-  Lemma wp_move_success_reg_samePC E pc_p pc_g pc_b pc_e pc_a pc_a' w pc_p' :
+  Lemma wp_move_success_reg_samePC E pc_p pc_b pc_e pc_a pc_a' w :
     decodeInstrW w = Mov PC (inr PC) →
-    PermFlows pc_p pc_p' →
-    isCorrectPC (inr ((pc_p,pc_g),pc_b,pc_e,pc_a)) →
+    isCorrectPC (inr (pc_p,pc_b,pc_e,pc_a)) →
     (pc_a + 1)%a = Some pc_a' →
 
-    {{{ ▷ PC ↦ᵣ inr ((pc_p,pc_g),pc_b,pc_e,pc_a)
-        ∗ ▷ pc_a ↦ₐ[pc_p'] w }}}
+    {{{ ▷ PC ↦ᵣ inr (pc_p,pc_b,pc_e,pc_a)
+        ∗ ▷ pc_a ↦ₐ w }}}
       Instr Executable @ E
       {{{ RET NextIV;
-          PC ↦ᵣ inr ((pc_p,pc_g),pc_b,pc_e,pc_a')
-          ∗ pc_a ↦ₐ[pc_p'] w }}}.
+          PC ↦ᵣ inr (pc_p,pc_b,pc_e,pc_a')
+          ∗ pc_a ↦ₐ w }}}.
   Proof.
-    iIntros (Hinstr Hfl Hvpc Hpca' ϕ) "(>HPC & >Hpc_a) Hφ".
+    iIntros (Hinstr Hvpc Hpca' ϕ) "(>HPC & >Hpc_a) Hφ".
     iDestruct (map_of_regs_1 with "HPC") as "Hmap".
     iApply (wp_Mov with "[$Hmap Hpc_a]"); eauto; simplify_map_eq; eauto.
     by unfold regs_of; rewrite !dom_insert; set_solver+.
@@ -213,22 +202,21 @@ Section cap_lang_rules.
       incrementPC_inv; simplify_map_eq; eauto. congruence. }
   Qed.
 
-  Lemma wp_move_success_reg_toPC E pc_p pc_g pc_b pc_e pc_a w r1 p g b e a a' pc_p' :
+  Lemma wp_move_success_reg_toPC E pc_p pc_b pc_e pc_a w r1 p b e a a':
     decodeInstrW w = Mov PC (inr r1) →
-    PermFlows pc_p pc_p' →
-    isCorrectPC (inr ((pc_p,pc_g),pc_b,pc_e,pc_a)) →
+    isCorrectPC (inr (pc_p,pc_b,pc_e,pc_a)) →
     (a + 1)%a = Some a' →
 
-    {{{ ▷ PC ↦ᵣ inr ((pc_p,pc_g),pc_b,pc_e,pc_a)
-        ∗ ▷ pc_a ↦ₐ[pc_p'] w
-        ∗ ▷ r1 ↦ᵣ inr ((p,g),b,e,a) }}}
+    {{{ ▷ PC ↦ᵣ inr (pc_p,pc_b,pc_e,pc_a)
+        ∗ ▷ pc_a ↦ₐ w
+        ∗ ▷ r1 ↦ᵣ inr (p,b,e,a) }}}
       Instr Executable @ E
       {{{ RET NextIV;
-          PC ↦ᵣ inr ((p,g),b,e,a')
-          ∗ pc_a ↦ₐ[pc_p'] w
-          ∗ r1 ↦ᵣ inr ((p,g),b,e,a) }}}.
+          PC ↦ᵣ inr (p,b,e,a')
+          ∗ pc_a ↦ₐ w
+          ∗ r1 ↦ᵣ inr (p,b,e,a) }}}.
   Proof.
-    iIntros (Hinstr Hfl Hvpc Hpca' ϕ) "(>HPC & >Hpc_a & >Hr1) Hφ".
+    iIntros (Hinstr Hvpc Hpca' ϕ) "(>HPC & >Hpc_a & >Hr1) Hφ".
     iDestruct (map_of_regs_2 with "HPC Hr1") as "[Hmap %]".
     iApply (wp_Mov with "[$Hmap Hpc_a]"); eauto; simplify_map_eq; eauto.
     by unfold regs_of; rewrite !dom_insert; set_solver+.
@@ -243,23 +231,21 @@ Section cap_lang_rules.
       incrementPC_inv; simplify_map_eq; eauto. congruence. }
   Qed.
 
-  Lemma wp_move_success_reg_fromPC E pc_p pc_g pc_b pc_e pc_a pc_a' w r1 wr1 pc_p' :
+  Lemma wp_move_success_reg_fromPC E pc_p pc_b pc_e pc_a pc_a' w r1 wr1 :
     decodeInstrW w = Mov r1 (inr PC) →
-    PermFlows pc_p pc_p' →
-    isCorrectPC (inr ((pc_p,pc_g),pc_b,pc_e,pc_a)) →
+    isCorrectPC (inr (pc_p,pc_b,pc_e,pc_a)) →
     (pc_a + 1)%a = Some pc_a' →
-    PC ≠ r1 →
 
-    {{{ ▷ PC ↦ᵣ inr ((pc_p,pc_g),pc_b,pc_e,pc_a)
-        ∗ ▷ pc_a ↦ₐ[pc_p'] w
+    {{{ ▷ PC ↦ᵣ inr (pc_p,pc_b,pc_e,pc_a)
+        ∗ ▷ pc_a ↦ₐ w
         ∗ ▷ r1 ↦ᵣ wr1 }}}
       Instr Executable @ E
       {{{ RET NextIV;
-          PC ↦ᵣ inr ((pc_p,pc_g),pc_b,pc_e,pc_a')
-          ∗ pc_a ↦ₐ[pc_p'] w
-          ∗ r1 ↦ᵣ inr ((pc_p,pc_g),pc_b,pc_e,pc_a) }}}.
+          PC ↦ᵣ inr (pc_p,pc_b,pc_e,pc_a')
+          ∗ pc_a ↦ₐ w
+          ∗ r1 ↦ᵣ inr (pc_p,pc_b,pc_e,pc_a) }}}.
   Proof.
-    iIntros (Hinstr Hfl Hvpc Hpca' Hne ϕ) "(>HPC & >Hpc_a & >Hr1) Hφ".
+    iIntros (Hinstr Hvpc Hpca' ϕ) "(>HPC & >Hpc_a & >Hr1) Hφ".
     iDestruct (map_of_regs_2 with "HPC Hr1") as "[Hmap %]".
     iApply (wp_Mov with "[$Hmap Hpc_a]"); eauto; simplify_map_eq; eauto.
     by unfold regs_of; rewrite !dom_insert; set_solver+.
