theories/rules/rules_Restrict.v
@@ -5,7 +5,7 @@ From iris.proofmode Require Import tactics.
 From iris.algebra Require Import frac.
 
 Section cap_lang_rules.
-  Context `{memG Σ, regG Σ, MonRef: MonRefG (leibnizO _) CapR_rtc Σ}.
+  Context `{memG Σ, regG Σ}.
   Context `{MachineParameters}.
   Implicit Types P Q : iProp Σ.
   Implicit Types σ : ExecConf.
@@ -20,74 +20,70 @@ Section cap_lang_rules.
   (* TODO: Move somewhere *)
   Ltac destruct_cap c :=
     let p := fresh "p" in
-    let g := fresh "g" in
     let b := fresh "b" in
     let e := fresh "e" in
     let a := fresh "a" in
-    destruct c as ((((p & g) & b) & e) & a).
+    destruct c as (((p & b) & e) & a).
 
   Inductive Restrict_failure (regs: Reg) (dst: RegName) (src: Z + RegName) :=
   | Restrict_fail_dst_noncap z:
       regs !! dst = Some (inl z) →
       Restrict_failure regs dst src
-  | Restrict_fail_pE p g b e a:
-      regs !! dst = Some (inr (p, g, b, e, a)) →
+  | Restrict_fail_pE p b e a:
+      regs !! dst = Some (inr (p, b, e, a)) →
       p = E →
       Restrict_failure regs dst src
   | Restrict_fail_src_nonz:
       z_of_argument regs src = None →
       Restrict_failure regs dst src
-  | Restrict_fail_invalid_perm p g b e a n:
-      regs !! dst = Some (inr (p, g, b, e, a)) →
+  | Restrict_fail_invalid_perm p b e a n:
+      regs !! dst = Some (inr (p, b, e, a)) →
       p ≠ E →
       z_of_argument regs src = Some n →
-      PermPairFlowsTo (decodePermPair n) (p, g) = false →
+      PermFlowsTo (decodePerm n) p = false →
       Restrict_failure regs dst src
-  | Restrict_fail_PC_overflow p g b e a n:
-      regs !! dst = Some (inr (p, g, b, e, a)) →
+  | Restrict_fail_PC_overflow p b e a n:
+      regs !! dst = Some (inr (p, b, e, a)) →
       p ≠ E →
       z_of_argument regs src = Some n →
-      PermPairFlowsTo (decodePermPair n) (p, g) = true →
-      incrementPC (<[ dst := inr (decodePermPair n, b, e, a) ]> regs) = None →
+      PermFlowsTo (decodePerm n) p = true →
+      incrementPC (<[ dst := inr (decodePerm n, b, e, a) ]> regs) = None →
       Restrict_failure regs dst src.
 
   Inductive Restrict_spec (regs: Reg) (dst: RegName) (src: Z + RegName) (regs': Reg): cap_lang.val -> Prop :=
-  | Restrict_spec_success p g b e a n:
-      regs !! dst = Some (inr (p, g, b, e, a)) →
+  | Restrict_spec_success p b e a n:
+      regs !! dst = Some (inr (p, b, e, a)) →
       p ≠ E ->
       z_of_argument regs src = Some n →
-      PermPairFlowsTo (decodePermPair n) (p, g) = true →
-      incrementPC (<[ dst := inr (decodePermPair n, b, e, a) ]> regs) = Some regs' →
+      PermFlowsTo (decodePerm n) p = true →
+      incrementPC (<[ dst := inr (decodePerm n, b, e, a) ]> regs) = Some regs' →
       Restrict_spec regs dst src regs' NextIV
   | Restrict_spec_failure:
       Restrict_failure regs dst src →
       Restrict_spec regs dst src regs' FailedV.
 
-  Lemma wp_Restrict Ep pc_p pc_g pc_b pc_e pc_a pc_p' w dst src regs :
+  Lemma wp_Restrict Ep pc_p pc_b pc_e pc_a w dst src regs :
     decodeInstrW w = Restrict dst src ->
-
-    PermFlows pc_p pc_p' →
-    isCorrectPC (inr ((pc_p, pc_g), pc_b, pc_e, pc_a)) →
-    regs !! PC = Some (inr ((pc_p, pc_g), pc_b, pc_e, pc_a)) →
+    isCorrectPC (inr (pc_p, pc_b, pc_e, pc_a)) →
+    regs !! PC = Some (inr (pc_p, pc_b, pc_e, pc_a)) →
     regs_of (Restrict dst src) ⊆ dom _ regs →
-    {{{ ▷ pc_a ↦ₐ[pc_p'] w ∗
+    
+    {{{ ▷ pc_a ↦ₐ w ∗
         ▷ [∗ map] k↦y ∈ regs, k ↦ᵣ y }}}
       Instr Executable @ Ep
     {{{ regs' retv, RET retv;
         ⌜ Restrict_spec regs dst src regs' retv ⌝ ∗
-        pc_a ↦ₐ[pc_p'] w ∗
+        pc_a ↦ₐ w ∗
         [∗ map] k↦y ∈ regs', k ↦ᵣ y }}}.
   Proof.
-    iIntros (Hinstr Hfl Hvpc HPC Dregs φ) "(>Hpc_a & >Hmap) Hφ".
+    iIntros (Hinstr Hvpc HPC Dregs φ) "(>Hpc_a & >Hmap) Hφ".
     iApply wp_lift_atomic_head_step_no_fork; auto.
     iIntros (σ1 l1 l2 n) "Hσ1 /=". destruct σ1; simpl.
     iDestruct "Hσ1" as "[Hr Hm]".
-    assert (pc_p' ≠ O).
-    { destruct pc_p'; auto. destruct pc_p; inversion Hfl. inversion Hvpc; naive_solver. }
     iDestruct (gen_heap_valid_inclSepM with "Hr Hmap") as %Hregs.
     have HPC' := regs_lookup_eq _ _ _ HPC.
     have ? := lookup_weaken _ _ _ _ HPC Hregs.
-    iDestruct (@gen_heap_valid_cap with "Hm Hpc_a") as %Hpc_a; auto.
+    iDestruct (@gen_heap_valid with "Hm Hpc_a") as %Hpc_a; auto.
     iModIntro. iSplitR. by iPureIntro; apply normal_always_head_reducible.
     iNext. iIntros (e2 σ2 efs Hpstep).
     apply prim_step_exec_inv in Hpstep as (-> & -> & (c & -> & Hstep)).
@@ -114,20 +110,20 @@ Section cap_lang_rules.
     { subst p. cbn in Hstep. rewrite /RegLocate Hdst in Hstep.
       repeat case_match; inv Hstep; iFailWP "Hφ" Restrict_fail_pE. }
 
-    destruct (PermPairFlowsTo (decodePermPair wsrc) (p, g)) eqn:Hflows; cycle 1.
+    destruct (PermFlowsTo (decodePerm wsrc) p) eqn:Hflows; cycle 1.
     { rewrite /= /RegLocate Hdst in Hstep.
       destruct Hwsrc as [ -> | (r0 & -> & Hr0 & Hr0') ].
       all: rewrite ?Hr0' Hflows in Hstep.
       all: repeat case_match; inv Hstep; iFailWP "Hφ" Restrict_fail_invalid_perm. }
 
-    assert ((c, σ2) = updatePC (update_reg (r, m) dst (inr (decodePermPair wsrc, b, e, a)))) as HH.
+    assert ((c, σ2) = updatePC (update_reg (r, m) dst (inr (decodePerm wsrc, b, e, a)))) as HH.
     { rewrite /= /RegLocate Hdst in Hstep.
       destruct Hwsrc as [ -> | (r0 & -> & Hr0 & Hr0') ].
       all: rewrite ?Hr0' Hflows in Hstep.
       all: repeat case_match; inv Hstep; eauto; congruence. }
     clear Hstep. rewrite /update_reg /= in HH.
 
-    destruct (incrementPC (<[ dst := inr (decodePermPair wsrc, b, e, a) ]> regs)) eqn:Hregs';
+    destruct (incrementPC (<[ dst := inr (decodePerm wsrc, b, e, a) ]> regs)) eqn:Hregs';
       pose proof Hregs' as H'regs'; cycle 1.
     { apply incrementPC_fail_updatePC with (m:=m) in Hregs'.
       eapply updatePC_fail_incl with (m':=m) in Hregs'.
@@ -138,7 +134,7 @@ Section cap_lang_rules.
       iFailWP "Hφ" Restrict_fail_PC_overflow. }
 
     eapply (incrementPC_success_updatePC _ m) in Hregs'
-      as (p' & g' & b' & e' & a'' & a_pc' & HPC'' & Ha_pc' & HuPC & ->).
+      as (p' & g' & b' & e' & a'' & a_pc' & HPC'' & HuPC & ->).
     eapply updatePC_success_incl with (m':=m) in HuPC. 2: by eapply insert_mono; eauto.
     simplify_pair_eq. iFrame.
     iMod ((gen_heap_update_inSepM _ _ dst) with "Hr Hmap") as "[Hr Hmap]"; eauto.
@@ -146,23 +142,22 @@ Section cap_lang_rules.
     iFrame. iApply "Hφ". iFrame. iPureIntro. econstructor; eauto.
   Qed.
 
-  Lemma wp_restrict_success_reg_PC Ep pc_p pc_g pc_b pc_e pc_a pc_a' w rv z a' pc_p' :
+  Lemma wp_restrict_success_reg_PC Ep pc_p pc_b pc_e pc_a pc_a' w rv z a' :
     decodeInstrW w = Restrict PC (inr rv) →
-    PermFlows pc_p pc_p' →
-    isCorrectPC (inr ((pc_p,pc_g),pc_b,pc_e,pc_a)) →
+    isCorrectPC (inr (pc_p,pc_b,pc_e,pc_a)) →
     (pc_a + 1)%a = Some pc_a' →
-    PermPairFlowsTo (decodePermPair z) (pc_p,pc_g) = true →
+    PermFlowsTo (decodePerm z) pc_p = true →
 
-     {{{ ▷ PC ↦ᵣ inr ((pc_p,pc_g),pc_b,pc_e,pc_a)
-         ∗ ▷ pc_a ↦ₐ[pc_p'] w
+     {{{ ▷ PC ↦ᵣ inr (pc_p,pc_b,pc_e,pc_a)
+         ∗ ▷ pc_a ↦ₐ w
          ∗ ▷ rv ↦ᵣ inl z }}}
        Instr Executable @ Ep
        {{{ RET NextIV;
-           PC ↦ᵣ inr (decodePermPair z,pc_b,pc_e,pc_a')
-           ∗ pc_a ↦ₐ[pc_p'] w
+           PC ↦ᵣ inr (decodePerm z,pc_b,pc_e,pc_a')
+           ∗ pc_a ↦ₐ w
            ∗ rv ↦ᵣ inl z }}}.
    Proof.
-     iIntros (Hinstr Hfl Hvpc Hpca' Hflows ϕ) "(>HPC & >Hpc_a & >Hrv) Hφ".
+     iIntros (Hinstr Hvpc Hpca' Hflows ϕ) "(>HPC & >Hpc_a & >Hrv) Hφ".
      iDestruct (map_of_regs_2 with "HPC Hrv") as "[Hmap %]".
      iApply (wp_Restrict with "[$Hmap Hpc_a]"); eauto; simplify_map_eq; eauto.
      by unfold regs_of; rewrite !dom_insert; set_solver+.
@@ -173,34 +168,33 @@ Section cap_lang_rules.
      destruct Hspec as [| * Hfail].
      { (* Success *)
        iApply "Hφ". iFrame. incrementPC_inv; simplify_map_eq.
-       destruct (decodePermPair n); simplify_eq. rewrite !insert_insert.
-       iDestruct (regs_of_map_2 with "Hmap") as "(?&?)"; eauto; iFrame. }
+       rewrite !insert_insert.
+       iDestruct (regs_of_map_2 with "Hmap") as "(?&?)"; eauto; iFrame.
+     }
      { (* Failure (contradiction) *)
        destruct Hfail; simplify_map_eq; eauto; try congruence.
        incrementPC_inv; simplify_map_eq; eauto. congruence. }
    Qed.
 
-   Lemma wp_restrict_success_reg Ep pc_p pc_g pc_b pc_e pc_a pc_a' w r1 rv p g b e a z
-         pc_p' :
+   Lemma wp_restrict_success_reg Ep pc_p pc_b pc_e pc_a pc_a' w r1 rv p b e a z :
      decodeInstrW w = Restrict r1 (inr rv) →
-     PermFlows pc_p pc_p' →
-     isCorrectPC (inr ((pc_p,pc_g),pc_b,pc_e,pc_a)) →
+     isCorrectPC (inr (pc_p,pc_b,pc_e,pc_a)) →
      (pc_a + 1)%a = Some pc_a' →
-     PermPairFlowsTo (decodePermPair z) (p,g) = true →
-     r1 ≠ PC → p ≠ E →
+     PermFlowsTo (decodePerm z) p = true →
+     p ≠ E →
 
-     {{{ ▷ PC ↦ᵣ inr ((pc_p,pc_g),pc_b,pc_e,pc_a)
-         ∗ ▷ pc_a ↦ₐ[pc_p'] w
-         ∗ ▷ r1 ↦ᵣ inr ((p,g),b,e,a)
+     {{{ ▷ PC ↦ᵣ inr (pc_p,pc_b,pc_e,pc_a)
+         ∗ ▷ pc_a ↦ₐ w
+         ∗ ▷ r1 ↦ᵣ inr (p,b,e,a)
          ∗ ▷ rv ↦ᵣ inl z }}}
        Instr Executable @ Ep
        {{{ RET NextIV;
-           PC ↦ᵣ inr ((pc_p,pc_g),pc_b,pc_e, pc_a')
-           ∗ pc_a ↦ₐ[pc_p'] w
+           PC ↦ᵣ inr (pc_p,pc_b,pc_e, pc_a')
+           ∗ pc_a ↦ₐ w
            ∗ rv ↦ᵣ inl z
-           ∗ r1 ↦ᵣ inr (decodePermPair z,b,e,a) }}}.
+           ∗ r1 ↦ᵣ inr (decodePerm z,b,e,a) }}}.
    Proof.
-     iIntros (Hinstr Hfl Hvpc Hpca' Hflows Hne1 Hnp ϕ) "(>HPC & >Hpc_a & >Hr1 & >Hrv) Hφ".
+     iIntros (Hinstr Hvpc Hpca' Hflows Hnp ϕ) "(>HPC & >Hpc_a & >Hr1 & >Hrv) Hφ".
      iDestruct (map_of_regs_3 with "HPC Hr1 Hrv") as "[Hmap (%&%&%)]".
      iApply (wp_Restrict with "[$Hmap Hpc_a]"); eauto; simplify_map_eq; eauto.
      by unfold regs_of; rewrite !dom_insert; set_solver+.
@@ -217,21 +211,20 @@ Section cap_lang_rules.
       incrementPC_inv; simplify_map_eq; eauto. congruence. }
    Qed.
 
-   Lemma wp_restrict_success_z_PC Ep pc_p pc_g pc_b pc_e pc_a pc_a' w z pc_p' :
+   Lemma wp_restrict_success_z_PC Ep pc_p pc_b pc_e pc_a pc_a' w z :
      decodeInstrW w = Restrict PC (inl z) →
-     PermFlows pc_p pc_p' →
-     isCorrectPC (inr ((pc_p,pc_g),pc_b,pc_e,pc_a)) →
+     isCorrectPC (inr (pc_p,pc_b,pc_e,pc_a)) →
      (pc_a + 1)%a = Some pc_a' →
-     PermPairFlowsTo (decodePermPair z) (pc_p,pc_g) = true →
+     PermFlowsTo (decodePerm z) pc_p = true →
 
-     {{{ ▷ PC ↦ᵣ inr ((pc_p,pc_g),pc_b,pc_e,pc_a)
-         ∗ ▷ pc_a ↦ₐ[pc_p'] w }}}
+     {{{ ▷ PC ↦ᵣ inr (pc_p,pc_b,pc_e,pc_a)
+         ∗ ▷ pc_a ↦ₐ w }}}
        Instr Executable @ Ep
      {{{ RET NextIV;
-         PC ↦ᵣ inr (decodePermPair z,pc_b,pc_e,pc_a')
-         ∗ pc_a ↦ₐ[pc_p'] w }}}.
+         PC ↦ᵣ inr (decodePerm z,pc_b,pc_e,pc_a')
+         ∗ pc_a ↦ₐ w }}}.
    Proof.
-     iIntros (Hinstr Hfl Hvpc Hpca' Hflows ϕ) "(>HPC & >Hpc_a) Hφ".
+     iIntros (Hinstr Hvpc Hpca' Hflows ϕ) "(>HPC & >Hpc_a) Hφ".
      iDestruct (map_of_regs_1 with "HPC") as "Hmap".
      iApply (wp_Restrict with "[$Hmap Hpc_a]"); eauto; simplify_map_eq; eauto.
      by rewrite !dom_insert; set_solver+.
@@ -243,31 +236,30 @@ Section cap_lang_rules.
      destruct Hspec as [ | * Hfail ].
      { (* Success *)
        iApply "Hφ". iFrame. incrementPC_inv; simplify_map_eq.
-       rewrite !insert_insert. destruct (decodePermPair n); simplify_eq.
+       rewrite !insert_insert.
        iApply (regs_of_map_1 with "Hmap"). }
      { (* Failure (contradiction) *)
        destruct Hfail; simplify_map_eq; eauto. congruence.
        incrementPC_inv; simplify_map_eq; eauto. congruence. }
    Qed.
 
-   Lemma wp_restrict_success_z Ep pc_p pc_g pc_b pc_e pc_a pc_a' w r1 p g b e a z pc_p' :
+   Lemma wp_restrict_success_z Ep pc_p pc_b pc_e pc_a pc_a' w r1 p b e a z :
      decodeInstrW w = Restrict r1 (inl z) →
-     PermFlows pc_p pc_p' →
-     isCorrectPC (inr ((pc_p,pc_g),pc_b,pc_e,pc_a)) →
+     isCorrectPC (inr (pc_p,pc_b,pc_e,pc_a)) →
      (pc_a + 1)%a = Some pc_a' →
-     PermPairFlowsTo (decodePermPair z) (p,g) = true →
-     r1 ≠ PC → p ≠ E →
+     PermFlowsTo (decodePerm z) p = true →
+     p ≠ E →
 
-     {{{ ▷ PC ↦ᵣ inr ((pc_p,pc_g),pc_b,pc_e,pc_a)
-         ∗ ▷ pc_a ↦ₐ[pc_p'] w
-         ∗ ▷ r1 ↦ᵣ inr ((p,g),b,e,a) }}}
+     {{{ ▷ PC ↦ᵣ inr (pc_p,pc_b,pc_e,pc_a)
+         ∗ ▷ pc_a ↦ₐ w
+         ∗ ▷ r1 ↦ᵣ inr (p,b,e,a) }}}
        Instr Executable @ Ep
      {{{ RET NextIV;
-         PC ↦ᵣ inr ((pc_p,pc_g),pc_b,pc_e,pc_a')
-         ∗ pc_a ↦ₐ[pc_p'] w
-         ∗ r1 ↦ᵣ inr (decodePermPair z,b,e,a) }}}.
+         PC ↦ᵣ inr (pc_p,pc_b,pc_e,pc_a')
+         ∗ pc_a ↦ₐ w
+         ∗ r1 ↦ᵣ inr (decodePerm z,b,e,a) }}}.
    Proof.
-     iIntros (Hinstr Hfl Hvpc Hpca' Hflows Hne1 HpE ϕ) "(>HPC & >Hpc_a & >Hr1) Hφ".
+     iIntros (Hinstr Hvpc Hpca' Hflows HpE ϕ) "(>HPC & >Hpc_a & >Hr1) Hφ".
      iDestruct (map_of_regs_2 with "HPC Hr1") as "[Hmap %]".
      iApply (wp_Restrict with "[$Hmap Hpc_a]"); eauto; simplify_map_eq; eauto.
      by unfold regs_of; rewrite !dom_insert; set_solver+.
@@ -278,7 +270,6 @@ Section cap_lang_rules.
      destruct Hspec as [| * Hfail].
      { (* Success *)
        iApply "Hφ". iFrame. incrementPC_inv; simplify_map_eq.
-       destruct (decodePermPair n); simplify_eq.
        rewrite (insert_commute _ PC r1) // insert_insert
                (insert_commute _ PC r1) // insert_insert.
        iDestruct (regs_of_map_2 with "Hmap") as "(?&?)"; eauto; iFrame. }
