theories/rules/rules_Store.v
@@ -1,11 +1,11 @@
-From cap_machine Require Import region_invariants rules_base.
+From cap_machine Require Import rules_base.
 From iris.base_logic Require Export invariants gen_heap.
 From iris.program_logic Require Export weakestpre ectx_lifting.
 From iris.proofmode Require Import tactics.
 From iris.algebra Require Import frac.
 
 Section cap_lang_rules.
-  Context `{memG Σ, regG Σ, MonRef: MonRefG (leibnizO _) CapR_rtc Σ}.
+  Context `{memG Σ, regG Σ}.
   Context `{MachineParameters}.
   Implicit Types P Q : iProp Σ.
   Implicit Types σ : ExecConf.
@@ -16,24 +16,6 @@ Section cap_lang_rules.
   Implicit Types w : Word.
   Implicit Types reg : gmap RegName Word.
   Implicit Types ms : gmap Addr Word.
-
-  Lemma wa_and_locality_allows_update (p p' : Perm) (storev : Word):
-      writeAllowed p = true
-      → PermFlows p p'
-      → (isLocalWord storev = false ∨ pwl p = true)
-      → PermFlows (LeastPermUpd storev) p'.
-  Proof.
-    intros Hwa HPFp HLocal.
-    destruct (isLocalWord storev) eqn:HiLW.
-    - apply isLocal_RWL in HiLW; rewrite HiLW.
-      destruct HLocal as [Hcontr | Hpwl]; first by exfalso.
-      apply pwl_implies_RWL_RWLX in Hpwl.
-      destruct Hpwl as [-> | ->]; eapply PermFlows_trans; eauto; econstructor.
-    - apply not_isLocal_WL in HiLW; rewrite HiLW.
-      cbv in Hwa.
-      refine (PermFlows_trans _ _ _ _ HPFp).
-      destruct p; cbv in Hwa; try congruence; done.
-  Qed.
 
   Definition word_of_argument (regs: Reg) (a: Z + RegName) : option Word :=
     match a with
@@ -57,24 +39,17 @@ Section cap_lang_rules.
          split; auto.
   Qed.
 
-  Definition reg_allows_store (regs : Reg) (r : RegName) p g b e a (storev : Word) :=
-    regs !! r = Some (inr ((p, g), b, e, a)) ∧
-    writeAllowed p = true ∧ withinBounds ((p, g), b, e, a) = true ∧
-    (isLocalWord storev = false ∨ pwl p = true).
+  Definition reg_allows_store (regs : Reg) (r : RegName) p b e a (storev : Word) :=
+    regs !! r = Some (inr (p, b, e, a)) ∧
+    writeAllowed p = true ∧ withinBounds (p, b, e, a) = true.
 
-  Inductive Store_failure (regs: Reg) (r1 : RegName)(r2 : Z + RegName) (mem : PermMem):=
+  Inductive Store_failure (regs: Reg) (r1 : RegName)(r2 : Z + RegName) (mem : gmap Addr Word):=
   | Store_fail_const z:
       regs !! r1 = Some(inl z) ->
       Store_failure regs r1 r2 mem
-  | Store_fail_bounds p g b e a:
-      regs !! r1 = Some(inr ((p, g), b, e, a)) ->
-      (writeAllowed p = false ∨ withinBounds ((p, g), b, e, a) = false) →
-      Store_failure regs r1 r2 mem
-  | Store_fail_invalid_locality p g b e a storev:
-      regs !! r1 = Some(inr ((p, g), b, e, a)) ->
-      word_of_argument regs r2 = Some storev ->
-      isLocalWord storev = true →
-      pwl p = false →
+  | Store_fail_bounds p b e a:
+      regs !! r1 = Some(inr (p, b, e, a)) ->
+      (writeAllowed p = false ∨ withinBounds (p, b, e, a) = false) →
       Store_failure regs r1 r2 mem
   | Store_fail_invalid_PC:
       incrementPC (regs) = None ->
@@ -83,13 +58,13 @@ Section cap_lang_rules.
 
   Inductive Store_spec
     (regs: Reg) (r1 : RegName) (r2 : Z + RegName)
-    (regs': Reg) (mem mem' : PermMem) : cap_lang.val → Prop
+    (regs': Reg) (mem mem' : gmap Addr Word) : cap_lang.val → Prop
   :=
-  | Store_spec_success p p' g b e a storev oldv :
+  | Store_spec_success p b e a storev oldv :
     word_of_argument regs r2 = Some storev ->
-    reg_allows_store regs r1 p g b e a storev  →
-    mem !! a = Some(p', oldv) →
-    mem' = (<[a := (p', storev)]> mem) →
+    reg_allows_store regs r1 p b e a storev  →
+    mem !! a = Some oldv →
+    mem' = (<[a := storev]> mem) →
     incrementPC(regs) = Some regs' ->
     Store_spec regs r1 r2 regs' mem mem' NextIV
   | Store_spec_failure :
@@ -97,27 +72,26 @@ Section cap_lang_rules.
     Store_spec regs r1 r2 regs' mem mem' FailedV.
 
 
-  Definition allow_store_map_or_true (r1 : RegName) (r2 : Z + RegName) (regs : Reg) (mem : PermMem):=
-    ∃ p g b e a storev,
-      read_reg_inr regs r1 p g b e a ∧ word_of_argument regs r2 = Some storev ∧
-      if decide (reg_allows_store regs r1 p g b e a storev) then
-        ∃ p' w, mem !! a = Some (p', w) ∧ PermFlows p p'
+  Definition allow_store_map_or_true (r1 : RegName) (r2 : Z + RegName) (regs : Reg) (mem : gmap Addr Word):=
+    ∃ p b e a storev,
+      read_reg_inr regs r1 p b e a ∧ word_of_argument regs r2 = Some storev ∧
+      if decide (reg_allows_store regs r1 p b e a storev) then
+        ∃ w, mem !! a = Some w
       else True.
 
   Lemma allow_store_implies_storev:
-    ∀ (r1 : RegName)(r2 : Z + RegName) (mem0 : PermMem) (r : Reg) (p : Perm) (g : Locality) (b e a : Addr) storev,
+    ∀ (r1 : RegName)(r2 : Z + RegName) (mem0 : gmap Addr Word) (r : Reg) (p : Perm) (b e a : Addr) storev,
       allow_store_map_or_true r1 r2 r mem0
-      → r !r! r1 = inr (p, g, b, e, a)
+      → r !r! r1 = inr (p, b, e, a)
       → word_of_argument r r2 = Some storev
       → writeAllowed p = true
-      → withinBounds (p, g, b, e, a) = true
-      → (isLocalWord storev = false ∨ pwl p = true)
-      → ∃ (p' : Perm) (storev : Word),
-          mem0 !! a = Some (p', storev) ∧ PermFlows p p'.
+      → withinBounds (p, b, e, a) = true
+      → ∃ (storev : Word),
+          mem0 !! a = Some storev.
   Proof.
-    intros r1 r2 mem0 r p g b e a storev HaStore Hr2v Hwoa Hwa Hwb HLocal.
+    intros r1 r2 mem0 r p b e a storev HaStore Hr2v Hwoa Hwa Hwb.
     unfold allow_store_map_or_true in HaStore.
-    destruct HaStore as (?&?&?&?&?&?&[Hrr | Hrl]&Hwo&Hmem).
+    destruct HaStore as (?&?&?&?&?&[Hrr | Hrl]&Hwo&Hmem).
     - assert (Hrr' := Hrr). option_locate_mr_once m r.
       rewrite Hrr1 in Hr2v; inversion Hr2v; subst.
       case_decide as HAL.
@@ -128,81 +102,72 @@ Section cap_lang_rules.
   Qed.
 
   Lemma mem_eq_implies_allow_store_map:
-    ∀ (regs : Reg)(mem : PermMem)(r1 : RegName)(r2 : Z + RegName)(w storev : Word) p g b e a
-      (p' : Perm)  ,
-      mem = <[a:=(p', w)]> ∅
-      → regs !! r1 = Some (inr (p,g,b,e,a))
-      → PermFlows p p'
+    ∀ (regs : Reg)(mem : gmap Addr Word)(r1 : RegName)(r2 : Z + RegName)(w storev : Word) p b e a,
+      mem = <[a:=w]> ∅
+      → regs !! r1 = Some (inr (p,b,e,a))
       → word_of_argument regs r2 = Some storev
       → allow_store_map_or_true r1 r2 regs mem.
   Proof.
-    intros regs mem r1 r2 w storev p g b e a p' Hmem Hrr2 Hpc_p' Hwoa.
-    exists p,g,b,e,a,storev; split.
+    intros regs mem r1 r2 w storev p b e a Hmem Hrr2 Hwoa.
+    exists p,b,e,a,storev; split.
     - left. by simplify_map_eq.
     - case_decide; last done.
-      split; auto. exists p', w. simplify_map_eq. auto.
+      split; auto. exists w. simplify_map_eq. auto.
   Qed.
 
   Lemma mem_neq_implies_allow_store_map:
-    ∀ (regs : Reg)(mem : PermMem)(r1 : RegName)(r2 : Z + RegName)(pc_a : Addr)
-      (w w' storev : Word) p g b e a
-      (pc_p' p' : Perm)  ,
+    ∀ (regs : Reg)(mem : gmap Addr Word)(r1 : RegName)(r2 : Z + RegName)(pc_a : Addr)
+      (w w' storev : Word) p b e a,
       a ≠ pc_a
-      → mem = <[pc_a:=(pc_p', w)]> (<[a:=(p', w')]> ∅)
-      → regs !! r1 = Some (inr (p,g,b,e,a))
-      → PermFlows p p'
+      → mem = <[pc_a:=w]> (<[a:=w']> ∅)
+      → regs !! r1 = Some (inr (p,b,e,a))
       → word_of_argument regs r2 = Some storev
       → allow_store_map_or_true r1 r2 regs mem.
   Proof.
-    intros regs mem r1 r2 pc_a w w' storev p g b e a pc_p' p' H4 Hrr2 Hp' Hpc_p' Hwoa.
-    exists p,g,b,e,a,storev; split.
+    intros regs mem r1 r2 pc_a w w' storev p b e a H4 Hrr2 Hwoa.
+    exists p,b,e,a,storev; split.
     - left. by simplify_map_eq.
     - case_decide; last done.
-      split; auto. exists p', w'. simplify_map_eq. split; auto.
+      split; auto. exists w'. simplify_map_eq. split; auto.
   Qed.
 
   Lemma mem_implies_allow_store_map:
-    ∀ (regs : Reg)(mem : PermMem)(r1 : RegName)(r2 : Z + RegName)(pc_a : Addr)
-      (w w' storev : Word) p g b e a
-      (pc_p' p' : Perm)  ,
+    ∀ (regs : Reg)(mem : gmap Addr Word)(r1 : RegName)(r2 : Z + RegName)(pc_a : Addr)
+      (w w' storev : Word) p b e a,
       (if (a =? pc_a)%a
-       then mem = <[pc_a:=(pc_p', w)]> ∅
-       else mem = <[pc_a:=(pc_p', w)]> (<[a:=(p', w')]> ∅))
-      → regs !! r1 = Some (inr (p,g,b,e,a))
-      → (if (a =? pc_a)%a then PermFlows p pc_p' else PermFlows p p')
+       then mem = <[pc_a:=w]> ∅
+       else mem = <[pc_a:=w]> (<[a:=w']> ∅))
+      → regs !! r1 = Some (inr (p,b,e,a))
       → word_of_argument regs r2 = Some storev
       → allow_store_map_or_true r1 r2 regs mem.
   Proof.
-    intros regs mem r1 r2 pc_a w w' storev p g b e a pc_p' p' H4 Hrr2 Hpf Hwoa.
+    intros regs mem r1 r2 pc_a w w' storev p b e a H4 Hrr2 Hwoa.
     destruct (a =? pc_a)%a eqn:Heq.
       + apply Z.eqb_eq, z_of_eq in Heq. subst a. eapply mem_eq_implies_allow_store_map; eauto.
       + apply Z.eqb_neq in Heq.  eapply mem_neq_implies_allow_store_map; eauto. congruence.
   Qed.
 
    Lemma wp_store Ep
-     pc_p pc_g pc_b pc_e pc_a pc_p'
+     pc_p pc_b pc_e pc_a
      r1 (r2 : Z + RegName) w mem regs :
    decodeInstrW w = Store r1 r2 →
-   PermFlows pc_p pc_p' →
-   isCorrectPC (inr ((pc_p, pc_g), pc_b, pc_e, pc_a)) →
-   regs !! PC = Some (inr ((pc_p, pc_g), pc_b, pc_e, pc_a)) →
+   isCorrectPC (inr (pc_p, pc_b, pc_e, pc_a)) →
+   regs !! PC = Some (inr (pc_p, pc_b, pc_e, pc_a)) →
    regs_of (Store r1 r2) ⊆ dom _ regs →
-   mem !! pc_a = Some (pc_p', w) →
+   mem !! pc_a = Some w →
    allow_store_map_or_true r1 r2 regs mem →
 
-   {{{ (▷ [∗ map] a↦pw ∈ mem, ∃ p w, ⌜pw = (p,w)⌝ ∗ a ↦ₐ[p] w) ∗
+   {{{ (▷ [∗ map] a↦w ∈ mem, a ↦ₐ w) ∗
        ▷ [∗ map] k↦y ∈ regs, k ↦ᵣ y }}}
      Instr Executable @ Ep
    {{{ regs' mem' retv, RET retv;
        ⌜ Store_spec regs r1 r2 regs' mem mem' retv⌝ ∗
-         ([∗ map] a↦pw ∈ mem', ∃ p w, ⌜pw = (p,w)⌝ ∗ a ↦ₐ[p] w) ∗
+         ([∗ map] a↦w ∈ mem', a ↦ₐ w) ∗
          [∗ map] k↦y ∈ regs', k ↦ᵣ y }}}.
    Proof.
-     iIntros (Hinstr Hfl Hvpc HPC Dregs Hmem_pc HaStore φ) "(>Hmem & >Hmap) Hφ".
+     iIntros (Hinstr Hvpc HPC Dregs Hmem_pc HaStore φ) "(>Hmem & >Hmap) Hφ".
      iApply wp_lift_atomic_head_step_no_fork; auto.
      iIntros (σ1 l1 l2 n) "[Hr Hm] /=". destruct σ1; simpl.
-     assert (pc_p' ≠ O).
-     { destruct pc_p'; auto. destruct pc_p; inversion Hfl. inversion Hvpc; naive_solver. }
      iDestruct (gen_heap_valid_inclSepM with "Hr Hmap") as %Hregs.
 
      (* Derive necessary register values in r *)
@@ -210,7 +175,7 @@ Section cap_lang_rules.
      specialize (indom_regs_incl _ _ _ Dregs Hregs) as Hri. unfold regs_of in Hri.
      feed destruct (Hri r1) as [r1v [Hr'1 Hr1]]. by set_solver+.
      pose proof (regs_lookup_eq _ _ _ Hr'1) as Hr''1.
-     iDestruct (gen_mem_valid_inSepM pc_a _ _ _ _ mem _ m with "Hm Hmem") as %Hma; eauto.
+     iDestruct (gen_mem_valid_inSepM pc_a _ _ _ mem _ m with "Hm Hmem") as %Hma; eauto.
 
      iModIntro.
      iSplitR. by iPureIntro; apply normal_always_head_reducible.
@@ -222,14 +187,14 @@ Section cap_lang_rules.
      cbn in Hstep. rewrite Hrr1 in Hstep.
 
      (* Now we start splitting on the different cases in the Load spec, and prove them one at a time *)
-     destruct r1v as  [| (([[p g] b] & e) & a) ] eqn:Hr1v.
+     destruct r1v as  [| (([p b] & e) & a) ] eqn:Hr1v.
      { (* Failure: r1 is not a capability *)
        assert (c = Failed ∧ σ2 = (r, m)) as (-> & ->)
          by (destruct r2; inversion Hstep; auto).
        iFailWP "Hφ" Store_fail_const.
      }
 
-     destruct (writeAllowed p && withinBounds ((p, g), b, e, a)) eqn:HWA; rewrite HWA in Hstep.
+     destruct (writeAllowed p && withinBounds (p, b, e, a)) eqn:HWA; rewrite HWA in Hstep.
      2 : { (* Failure: r2 is either not within bounds or doesnt allow reading *)
         assert (c = Failed ∧ σ2 = (r, m)) as (-> & ->)
          by (destruct r2; inversion Hstep; auto).
@@ -246,41 +211,17 @@ Section cap_lang_rules.
          cbn in HSV. rewrite Hr0 in HSV. inversion HSV.
      }
      assert (word_of_argument r r2 = Some(storev)) as HSVr.
-     { destruct r2; cbn in HSV. inversion HSV; by rewrite H4.
+     { destruct r2; cbn in HSV. inversion HSV; by rewrite H3.
        destruct (Hri r0) as [r0v [Hregs0 Hr0] ].  by set_solver+.
        rewrite -Hr0 in Hregs0; rewrite Hregs0 in HSV. exact HSV.
      }
 
-     destruct (decide (isLocalWord storev = true ∧ pwl p = false)).
-     {  (* Failure: trying to write a local value to a non-WL cap *)
-            destruct a0 as [HLW Hpwl].
-       assert (c = Failed ∧ σ2 = (r, m)) as (-> & ->).
-      { destruct storev.
-       - cbv in HLW; by exfalso.
-       - destruct (word_of_argument_inr _ _ _ HSVr) as (r0 & -> & Hr0s).
-         destruct (isLocalWord_cap_isLocal _ HLW) as (p' & g' & b' & e' & a' & -> & HIL).
-         option_locate_mr m r. rewrite /canStore Hrr0 HIL in Hstep.
-         destruct p; try by exfalso. all: by inversion Hstep.
-      }
-      iFailWP "Hφ" Store_fail_invalid_locality.
-     }
-
-     assert (isLocalWord storev = false ∨ pwl p = true) as HLocal.
-     {
-     apply (not_and_r) in n0.
-     destruct n0 as [Hlw | Hpwl].
-     destruct (isLocalWord storev); first by exfalso. by left.
-     destruct (pwl p); last by exfalso. by right.
-     } clear n0.
-
      (* Prove that a is in the memory map now, otherwise we cannot continue *)
-     pose proof (allow_store_implies_storev r1 r2 mem regs p g b e a storev) as (p' & oldv & Hmema & HPFp); auto.
+     pose proof (allow_store_implies_storev r1 r2 mem regs p b e a storev) as (oldv & Hmema); auto.
 
      (* Given this, prove that a is also present in the memory itself *)
-     iDestruct (mem_v_implies_m_v mem m p g b e a p' oldv with "Hmem Hm" ) as %Hma ; auto. by apply (writeAllowed_nonO p p').
+     iDestruct (mem_v_implies_m_v mem m b e a oldv with "Hmem Hm" ) as %Hma ; auto.
 
-     (* Prove that p' gives us sufficient permissions to update the memory *)
-     pose proof (wa_and_locality_allows_update p p' storev Hwa HPFp HLocal) as HLoadA.
      (* Regardless of whether we increment the PC, the memory will change: destruct on the PC later *)
      assert (updatePC (update_mem (r, m) a storev) = (c, σ2)) as HH.
       { destruct r2.
@@ -292,16 +233,9 @@ Section cap_lang_rules.
            simpl in HSVr; rewrite Hr0' in HSVr.
            inversion HSVr; subst storev. done.
          * destruct_cap c0.
-           epose proof (regs_lookup_inr_eq r r0 _ _ _ _ _ Hr0) as Hr0'.
-           simpl in HSVr; rewrite Hr0' in HSVr; inversion HSVr.
-           subst storev; clear HSVr.
-           destruct HLocal as [HiLW | Hpwl].
-           + cbv in HiLW. destruct c4; last by exfalso. simpl in Hstep. done.
-           + destruct c4; simpl in Hstep.
-             ++ done.
-             ++ apply pwl_implies_RWL_RWLX in Hpwl.
-                destruct Hpwl as [-> | ->]; done.
-       }
+           epose proof (regs_lookup_inr_eq r r0 _ _ _ _ Hr0) as Hr0'. 
+           simpl in HSVr; rewrite Hr0' in HSVr; inversion HSVr. auto. 
+      }
       iMod ((gen_mem_update_inSepM _ _ a) with "Hm Hmem") as "[Hm Hmem]"; eauto.
 
       destruct (incrementPC regs ) as [ regs' |] eqn:Hregs'.
@@ -316,7 +250,7 @@ Section cap_lang_rules.
      (* Success *)
       clear Hstep. rewrite /update_mem /= in HH.
       eapply (incrementPC_success_updatePC _ (<[a:=storev]> m)) in Hregs'
-        as (p1 & g1 & b1 & e1 & a1 & a_pc1 & HPC'' & Ha_pc' & HuPC & ->).
+        as (p1 & g1 & b1 & e1 & a1 & a_pc1 & HPC'' & HuPC & ->).
       eapply (updatePC_success_incl _ (<[a:=storev]> m)) in HuPC. 2: by eauto.
       rewrite HuPC in HH; clear HuPC; inversion HH; clear HH; subst c σ2. cbn.
 
@@ -325,25 +259,24 @@ Section cap_lang_rules.
       iFrame. iModIntro. iApply "Hφ". iFrame.
       iPureIntro. eapply Store_spec_success; eauto.
         * split; auto. exact Hr'1. all: auto.
-        * unfold incrementPC. by rewrite HPC'' Ha_pc'.
+        * unfold incrementPC. rewrite a_pc1 HPC''. 
       Unshelve. all: auto.
    Qed.
 
-  Lemma wp_store_success_z_PC E pc_p pc_p' pc_g pc_b pc_e pc_a pc_a' w z :
+  Lemma wp_store_success_z_PC E pc_p pc_b pc_e pc_a pc_a' w z :
      decodeInstrW w = Store PC (inl z) →
-     PermFlows pc_p pc_p' →
-     isCorrectPC (inr ((pc_p,pc_g),pc_b,pc_e,pc_a)) →
+     isCorrectPC (inr (pc_p,pc_b,pc_e,pc_a)) →
      (pc_a + 1)%a = Some pc_a' →
      writeAllowed pc_p = true →
 
-     {{{ ▷ PC ↦ᵣ inr ((pc_p,pc_g),pc_b,pc_e,pc_a)
-           ∗ ▷ pc_a ↦ₐ[pc_p'] w }}}
+     {{{ ▷ PC ↦ᵣ inr (pc_p,pc_b,pc_e,pc_a)
+           ∗ ▷ pc_a ↦ₐ w }}}
        Instr Executable @ E
        {{{ RET NextIV;
-           PC ↦ᵣ inr ((pc_p,pc_g),pc_b,pc_e,pc_a')
-              ∗ pc_a ↦ₐ[pc_p'] (inl z) }}}.
+           PC ↦ᵣ inr (pc_p,pc_b,pc_e,pc_a')
+              ∗ pc_a ↦ₐ (inl z) }}}.
   Proof.
-    iIntros (Hinstr Hfl Hvpc Hpca' Hwa φ)
+    iIntros (Hinstr Hvpc Hpca' Hwa φ)
             "(>HPC & >Hi) Hφ".
     iDestruct (map_of_regs_1 with "HPC") as "Hmap".
     iDestruct (memMap_resource_1 with "Hi") as "Hmem".
@@ -370,24 +303,22 @@ Section cap_lang_rules.
      }
    Qed.
 
-   Lemma wp_store_success_reg_PC E src wsrc pc_p pc_p' pc_g pc_b pc_e pc_a pc_a' w :
+   Lemma wp_store_success_reg_PC E src wsrc pc_p pc_b pc_e pc_a pc_a' w :
      decodeInstrW w = Store PC (inr src) →
-     PermFlows pc_p pc_p' →
-     isCorrectPC (inr ((pc_p,pc_g),pc_b,pc_e,pc_a)) →
+     isCorrectPC (inr (pc_p,pc_b,pc_e,pc_a)) →
      (pc_a + 1)%a = Some pc_a' →
      writeAllowed pc_p = true →
-     (isLocalWord wsrc = false ∨ (pc_p = RWL ∨ pc_p = RWLX)) ->
 
-     {{{ ▷ PC ↦ᵣ inr ((pc_p,pc_g),pc_b,pc_e,pc_a)
-           ∗ ▷ pc_a ↦ₐ[pc_p'] w
+     {{{ ▷ PC ↦ᵣ inr (pc_p,pc_b,pc_e,pc_a)
+           ∗ ▷ pc_a ↦ₐ w
            ∗ ▷ src ↦ᵣ wsrc }}}
        Instr Executable @ E
        {{{ RET NextIV;
-           PC ↦ᵣ inr ((pc_p,pc_g),pc_b,pc_e,pc_a')
-              ∗ pc_a ↦ₐ[pc_p'] wsrc
+           PC ↦ᵣ inr (pc_p,pc_b,pc_e,pc_a')
+              ∗ pc_a ↦ₐ wsrc
               ∗ src ↦ᵣ wsrc }}}.
    Proof.
-     iIntros (Hinstr Hfl Hvpc Hpca' Hwa Hloc φ)
+     iIntros (Hinstr Hvpc Hpca' Hwa φ)
             "(>HPC & >Hi & >Hsrc) Hφ".
      iDestruct (map_of_regs_2 with "HPC Hsrc") as "[Hmap %]".
      iDestruct (memMap_resource_1 with "Hi") as "Hmem".
@@ -412,27 +343,24 @@ Section cap_lang_rules.
        destruct Hfail; try incrementPC_inv; simplify_map_eq; eauto.
        - apply isCorrectPC_ra_wb in Hvpc. apply andb_prop_elim in Hvpc as [_ Hwb].
          destruct o; last apply Is_true_false in H3; congruence.
-       - destruct Hloc; first congruence. naive_solver.
-       - congruence.
+       - naive_solver. 
      }
     Qed.
 
-   Lemma wp_store_success_reg_PC_same E pc_p pc_g pc_b pc_e pc_a pc_a' w w' pc_p' :
+   Lemma wp_store_success_reg_PC_same E pc_p pc_b pc_e pc_a pc_a' w w' :
      decodeInstrW w = Store PC (inr PC) →
-     PermFlows pc_p pc_p' →
-     isCorrectPC (inr ((pc_p,pc_g),pc_b,pc_e,pc_a)) →
+     isCorrectPC (inr (pc_p,pc_b,pc_e,pc_a)) →
      (pc_a + 1)%a = Some pc_a' →
      writeAllowed pc_p = true →
-     (isLocal pc_g = false ∨ (pc_p = RWLX ∨ pc_p = RWL)) →
 
-     {{{ ▷ PC ↦ᵣ inr ((pc_p,pc_g),pc_b,pc_e,pc_a)
-           ∗ ▷ pc_a ↦ₐ[pc_p'] w }}}
+     {{{ ▷ PC ↦ᵣ inr (pc_p,pc_b,pc_e,pc_a)
+           ∗ ▷ pc_a ↦ₐ w }}}
        Instr Executable @ E
        {{{ RET NextIV;
-           PC ↦ᵣ inr ((pc_p,pc_g),pc_b,pc_e,pc_a')
-              ∗ pc_a ↦ₐ[pc_p'] inr ((pc_p,pc_g),pc_b,pc_e,pc_a) }}}.
+           PC ↦ᵣ inr (pc_p,pc_b,pc_e,pc_a')
+              ∗ pc_a ↦ₐ inr (pc_p,pc_b,pc_e,pc_a) }}}.
    Proof.
-     iIntros (Hinstr Hfl Hvpc Hpca' Hwa Hloc φ)
+     iIntros (Hinstr Hvpc Hpca' Hwa φ)
             "(>HPC & >Hi) Hφ".
      iDestruct (map_of_regs_1 with "HPC") as "Hmap".
      iDestruct (memMap_resource_1 with "Hi") as "Hmem".
@@ -457,29 +385,26 @@ Section cap_lang_rules.
        destruct Hfail; try incrementPC_inv; simplify_map_eq; eauto. destruct o . all: try congruence.
        - apply isCorrectPC_ra_wb in Hvpc. apply andb_prop_elim in Hvpc as [_ Hwb].
          apply Is_true_false in H2; congruence.
-       - destruct Hloc; first congruence. naive_solver.
      }
     Qed.
 
-   Lemma wp_store_success_same E pc_p pc_g pc_b pc_e pc_a pc_a' w dst z w'
-         p g b e pc_p' :
+   Lemma wp_store_success_same E pc_p pc_b pc_e pc_a pc_a' w dst z w'
+         p b e :
      decodeInstrW w = Store dst (inl z) →
-     PermFlows pc_p pc_p' →
-     PermFlows p pc_p' →
-     isCorrectPC (inr ((pc_p,pc_g),pc_b,pc_e,pc_a)) →
+     isCorrectPC (inr (pc_p,pc_b,pc_e,pc_a)) →
      (pc_a + 1)%a = Some pc_a' →
-     writeAllowed p = true ∧ withinBounds ((p, g), b, e, pc_a) = true →
+     writeAllowed p = true ∧ withinBounds (p, b, e, pc_a) = true →
 
-     {{{ ▷ PC ↦ᵣ inr ((pc_p,pc_g),pc_b,pc_e,pc_a)
-           ∗ ▷ pc_a ↦ₐ[pc_p'] w
-           ∗ ▷ dst ↦ᵣ inr ((p,g),b,e,pc_a) }}}
+     {{{ ▷ PC ↦ᵣ inr (pc_p,pc_b,pc_e,pc_a)
+           ∗ ▷ pc_a ↦ₐ w
+           ∗ ▷ dst ↦ᵣ inr (p,b,e,pc_a) }}}
        Instr Executable @ E
        {{{ RET NextIV;
-           PC ↦ᵣ inr ((pc_p,pc_g),pc_b,pc_e,pc_a')
-              ∗ pc_a ↦ₐ[pc_p'] (inl z)
-              ∗ dst ↦ᵣ inr ((p,g),b,e,pc_a) }}}.
+           PC ↦ᵣ inr (pc_p,pc_b,pc_e,pc_a')
+              ∗ pc_a ↦ₐ (inl z)
+              ∗ dst ↦ᵣ inr (p,b,e,pc_a) }}}.
     Proof.
-     iIntros (Hinstr Hfl Hfl' Hvpc Hpca' [Hwa Hwb] φ)
+     iIntros (Hinstr Hvpc Hpca' [Hwa Hwb] φ)
             "(>HPC & >Hi & >Hdst) Hφ".
      iDestruct (map_of_regs_2 with "HPC Hdst") as "[Hmap %]".
      iDestruct (memMap_resource_1 with "Hi") as "Hmem".
@@ -506,39 +431,34 @@ Section cap_lang_rules.
      }
      Qed.
 
-   Lemma wp_store_success_reg' E pc_p pc_g pc_b pc_e pc_a pc_a' w dst w'
-         p g b e a pc_p' p' :
+   Lemma wp_store_success_reg' E pc_p pc_b pc_e pc_a pc_a' w dst w'
+         p b e a :
       decodeInstrW w = Store dst (inr PC) →
-      PermFlows pc_p pc_p' →
-     isCorrectPC (inr ((pc_p,pc_g),pc_b,pc_e,pc_a)) →
+     isCorrectPC (inr (pc_p,pc_b,pc_e,pc_a)) →
      (pc_a + 1)%a = Some pc_a' →
-     writeAllowed p = true ∧ withinBounds ((p, g), b, e, a) = true →
-     (isLocal pc_g = false ∨ (p = RWLX ∨ p = RWL)) →
+     writeAllowed p = true ∧ withinBounds (p, b, e, a) = true →
 
-     {{{ ▷ PC ↦ᵣ inr ((pc_p,pc_g),pc_b,pc_e,pc_a)
-           ∗ ▷ pc_a ↦ₐ[pc_p'] w
-           ∗ ▷ dst ↦ᵣ inr ((p,g),b,e,a)
+     {{{ ▷ PC ↦ᵣ inr (pc_p,pc_b,pc_e,pc_a)
+           ∗ ▷ pc_a ↦ₐ w
+           ∗ ▷ dst ↦ᵣ inr (p,b,e,a)
            ∗ if (a =? pc_a)%a
-             then ⌜PermFlows p pc_p'⌝
-             else ⌜PermFlows p p'⌝ ∗ ▷ a ↦ₐ[p'] w' }}}
+             then emp
+             else ▷ a ↦ₐ w' }}}
        Instr Executable @ E
        {{{ RET NextIV;
-           PC ↦ᵣ inr ((pc_p,pc_g),pc_b,pc_e,pc_a')
-              ∗ pc_a ↦ₐ[pc_p'] (if (a =? pc_a)%a
-                               then (inr ((pc_p,pc_g),pc_b,pc_e,pc_a))
-                               else w)
-              ∗ dst ↦ᵣ inr ((p,g),b,e,a)
+           PC ↦ᵣ inr (pc_p,pc_b,pc_e,pc_a')
+              ∗ pc_a ↦ₐ (if (a =? pc_a)%a
+                         then (inr (pc_p,pc_b,pc_e,pc_a))
+                         else w)
+              ∗ dst ↦ᵣ inr (p,b,e,a)
               ∗ if (a =? pc_a)%a
                 then emp
-                else a ↦ₐ[p'] (inr ((pc_p,pc_g),pc_b,pc_e,pc_a)) }}}.
+                else a ↦ₐ (inr (pc_p,pc_b,pc_e,pc_a)) }}}.
    Proof.
-     iIntros (Hinstr Hfl Hvpc Hpca' [Hwa Hwb] Hloc φ)
+     iIntros (Hinstr Hvpc Hpca' [Hwa Hwb] φ)
             "(>HPC & >Hi & >Hdst & Ha) Hφ".
      iDestruct (map_of_regs_2 with "HPC Hdst") as "[Hmap %]".
-     iDestruct (extract_sep_if_split with "Ha") as "[Hflt Hr1a]".
-     iAssert (⌜if (a =? pc_a)%a then PermFlows p pc_p' else PermFlows p p'⌝)%I with "[Hflt]" as %Hfl'.
-     { iRevert "Hflt". destruct (a =? pc_a)%a; auto. }
-     iDestruct (memMap_resource_2gen_clater with "Hi Hr1a") as (mem) "[>Hmem %]".
+     iDestruct (memMap_resource_2gen_clater with "Hi Ha") as (mem) "[>Hmem %]".
 
     iApply (wp_store with "[$Hmap $Hmem]"); eauto; simplify_map_eq; eauto.
     { by rewrite !dom_insert; set_solver+. }
@@ -570,30 +490,26 @@ Section cap_lang_rules.
      { (* Failure (contradiction) *)
        destruct Hfail; try incrementPC_inv; simplify_map_eq; eauto.
        destruct o. all: try congruence.
-       destruct Hloc; first congruence. naive_solver.
      }
-     Qed.
+   Qed.
 
-   Lemma wp_store_success_reg_same' E pc_p pc_g pc_b pc_e pc_a pc_a' w dst
-         p g b e pc_p' :
+   Lemma wp_store_success_reg_same' E pc_p pc_b pc_e pc_a pc_a' w dst
+         p b e :
      decodeInstrW w = Store dst (inr dst) →
-     PermFlows pc_p pc_p' →
-     PermFlows p pc_p' →
-     isCorrectPC (inr ((pc_p,pc_g),pc_b,pc_e,pc_a)) →
+     isCorrectPC (inr (pc_p,pc_b,pc_e,pc_a)) →
      (pc_a + 1)%a = Some pc_a' →
-     writeAllowed p = true ∧ withinBounds ((p, g), b, e, pc_a) = true →
-     (isLocal g = false ∨ (p = RWLX ∨ p = RWL)) →
+     writeAllowed p = true ∧ withinBounds (p, b, e, pc_a) = true →
 
-     {{{ ▷ PC ↦ᵣ inr ((pc_p,pc_g),pc_b,pc_e,pc_a)
-           ∗ ▷ pc_a ↦ₐ[pc_p'] w
-           ∗ ▷ dst ↦ᵣ inr ((p,g),b,e,pc_a) }}}
+     {{{ ▷ PC ↦ᵣ inr (pc_p,pc_b,pc_e,pc_a)
+           ∗ ▷ pc_a ↦ₐ w
+           ∗ ▷ dst ↦ᵣ inr (p,b,e,pc_a) }}}
        Instr Executable @ E
        {{{ RET NextIV;
-           PC ↦ᵣ inr ((pc_p,pc_g),pc_b,pc_e,pc_a')
-              ∗ pc_a ↦ₐ[pc_p'] inr (p, g, b, e, pc_a)
-              ∗ dst ↦ᵣ inr ((p,g),b,e,pc_a) }}}.
+           PC ↦ᵣ inr (pc_p,pc_b,pc_e,pc_a')
+              ∗ pc_a ↦ₐ inr (p, b, e, pc_a)
+              ∗ dst ↦ᵣ inr (p,b,e,pc_a) }}}.
    Proof.
-     iIntros (Hinstr Hfl Hfl' Hvpc Hpca' [Hwa Hwb] Hloc φ)
+     iIntros (Hinstr Hvpc Hpca' [Hwa Hwb] φ)
             "(>HPC & >Hi & >Hdst) Hφ".
      iDestruct (map_of_regs_2 with "HPC Hdst") as "[Hmap %]".
      iDestruct (memMap_resource_1 with "Hi") as "Hmem".
@@ -617,32 +533,28 @@ Section cap_lang_rules.
      { (* Failure (contradiction) *)
        destruct Hfail; try incrementPC_inv; simplify_map_eq; eauto.
        destruct o. all: try congruence.
-       destruct Hloc; first congruence. naive_solver.
      }
    Qed.
 
-   Lemma wp_store_success_reg_same_a E pc_p pc_g pc_b pc_e pc_a pc_a' w dst src
-         p g b e pc_p' w'' :
+   Lemma wp_store_success_reg_same_a E pc_p pc_b pc_e pc_a pc_a' w dst src
+         p b e w'' :
       decodeInstrW w = Store dst (inr src) →
-      PermFlows pc_p pc_p' →
-      PermFlows p pc_p' →
-     isCorrectPC (inr ((pc_p,pc_g),pc_b,pc_e,pc_a)) →
+     isCorrectPC (inr (pc_p,pc_b,pc_e,pc_a)) →
      (pc_a + 1)%a = Some pc_a' →
-     writeAllowed p = true ∧ withinBounds ((p, g), b, e, pc_a) = true →
-     (isLocalWord w'' = false ∨ (p = RWLX ∨ p = RWL)) →
+     writeAllowed p = true ∧ withinBounds (p, b, e, pc_a) = true →
 
-     {{{ ▷ PC ↦ᵣ inr ((pc_p,pc_g),pc_b,pc_e,pc_a)
-           ∗ ▷ pc_a ↦ₐ[pc_p'] w
+     {{{ ▷ PC ↦ᵣ inr (pc_p,pc_b,pc_e,pc_a)
+           ∗ ▷ pc_a ↦ₐ w
            ∗ ▷ src ↦ᵣ w''
-           ∗ ▷ dst ↦ᵣ inr ((p,g),b,e,pc_a) }}}
+           ∗ ▷ dst ↦ᵣ inr (p,b,e,pc_a) }}}
        Instr Executable @ E
        {{{ RET NextIV;
-           PC ↦ᵣ inr ((pc_p,pc_g),pc_b,pc_e,pc_a')
-              ∗ pc_a ↦ₐ[pc_p'] w''
+           PC ↦ᵣ inr (pc_p,pc_b,pc_e,pc_a')
+              ∗ pc_a ↦ₐ w''
               ∗ src ↦ᵣ w''
-              ∗ dst ↦ᵣ inr ((p,g),b,e,pc_a)}}}.
+              ∗ dst ↦ᵣ inr (p,b,e,pc_a)}}}.
    Proof.
-     iIntros (Hinstr Hfl Hfl' Hvpc Hpca' [Hwa Hwb] Hloc φ)
+     iIntros (Hinstr Hvpc Hpca' [Hwa Hwb] φ)
              "(>HPC & >Hi & >Hsrc & >Hdst) Hφ".
      iDestruct (map_of_regs_3 with "HPC Hsrc Hdst") as "[Hmap (%&%&%)]".
      iDestruct (memMap_resource_1 with "Hi") as "Hmem".
@@ -666,149 +578,37 @@ Section cap_lang_rules.
      { (* Failure (contradiction) *)
        destruct Hfail; try incrementPC_inv; simplify_map_eq; eauto.
        destruct o. all: try congruence.
-       destruct Hloc; first congruence. naive_solver.
      }
    Qed.
 
-  Lemma wp_store_success_local_reg E pc_p pc_g pc_b pc_e pc_a pc_a' w dst src w'
-         p g b e a p' g' b' e' a' pc_p' p'' :
-    decodeInstrW w = Store dst (inr src) →
-    PermFlows pc_p pc_p' →
-    PermFlows p p'' →
-     isCorrectPC (inr ((pc_p,pc_g),pc_b,pc_e,pc_a)) →
-     (pc_a + 1)%a = Some pc_a' →
-     writeAllowed p = true ∧ withinBounds ((p, g), b, e, a) = true →
-     isLocal g' = true ∧ (p = RWLX ∨ p = RWL) →
-
-     {{{ ▷ PC ↦ᵣ inr ((pc_p,pc_g),pc_b,pc_e,pc_a)
-           ∗ ▷ pc_a ↦ₐ[pc_p'] w
-           ∗ ▷ src ↦ᵣ inr ((p',g'),b',e',a')
-           ∗ ▷ dst ↦ᵣ inr ((p,g),b,e,a)
-           ∗ ▷ a ↦ₐ[p''] w' }}}
-       Instr Executable @ E
-       {{{ RET NextIV;
-           PC ↦ᵣ inr ((pc_p,pc_g),pc_b,pc_e,pc_a')
-              ∗ pc_a ↦ₐ[pc_p'] w
-              ∗ src ↦ᵣ inr ((p',g'),b',e',a')
-              ∗ dst ↦ᵣ inr ((p,g),b,e,a)
-              ∗ a ↦ₐ[p''] inr ((p',g'),b',e',a') }}}.
-  Proof.
-    iIntros (Hinstr Hfl Hfl' Hvpc Hpca' [Hwa Hwb] Hloc φ)
-             "(>HPC & >Hi & >Hsrc & >Hdst & >Hsrca) Hφ".
-    iDestruct (map_of_regs_3 with "HPC Hsrc Hdst") as "[Hmap (%&%&%)]".
-    pose proof (writeAllowed_nonO _ _ Hfl' Hwa) as Hp''.
-    pose proof (correctPC_nonO _ _ _ _ _ _ Hfl Hvpc) as Hpc_p'.
-    iDestruct (memMap_resource_2ne_apply with "Hi Hsrca") as "[Hmem %]"; auto.
-
-    iApply (wp_store _ pc_p with "[$Hmap $Hmem]"); eauto; simplify_map_eq; eauto.
-    { by rewrite !dom_insert; set_solver+. }
-    { eapply mem_neq_implies_allow_store_map with (a := a) (p' := p''); eauto.
-      all: by simplify_map_eq. }
-    iNext. iIntros (regs' mem' retv) "(#Hspec & Hmem & Hmap)".
-    iDestruct "Hspec" as %Hspec.
-
-    destruct Hspec as [ | * Hfail ].
-     { (* Success *)
-       iApply "Hφ".
-       destruct H7 as [Hrr2 _]. simplify_map_eq.
-       rewrite insert_commute // insert_insert.
-       iDestruct (memMap_resource_2ne with "Hmem") as "[Hpc_a Ha]";auto.
-       incrementPC_inv.
-       simplify_map_eq.
-       rewrite insert_insert.
-       iDestruct (regs_of_map_3 with "[$Hmap]") as "[HPC [Hsrc Hdst] ]"; eauto. iFrame. }
-     { (* Failure (contradiction) *)
-       destruct Hfail; try incrementPC_inv; simplify_map_eq; eauto.
-       destruct o. all: try congruence.
-       destruct Hloc as [_ Hpwl]. naive_solver.
-     }
-  Qed.
-
-   Lemma wp_store_success_z_reg E pc_p pc_g pc_b pc_e pc_a pc_a' w dst src w'
-         p g b e a z pc_p' p' :
-     decodeInstrW w = Store dst (inr src) →
-     PermFlows pc_p pc_p' →
-     PermFlows p p' →
-     isCorrectPC (inr ((pc_p,pc_g),pc_b,pc_e,pc_a)) →
-     (pc_a + 1)%a = Some pc_a' →
-     writeAllowed p = true ∧ withinBounds ((p, g), b, e, a) = true →
-
-     {{{ ▷ PC ↦ᵣ inr ((pc_p,pc_g),pc_b,pc_e,pc_a)
-           ∗ ▷ pc_a ↦ₐ[pc_p'] w
-           ∗ ▷ src ↦ᵣ inl z
-           ∗ ▷ dst ↦ᵣ inr ((p,g),b,e,a)
-           ∗ ▷ a ↦ₐ[p'] w' }}}
-       Instr Executable @ E
-       {{{ RET NextIV;
-           PC ↦ᵣ inr ((pc_p,pc_g),pc_b,pc_e,pc_a')
-              ∗ pc_a ↦ₐ[pc_p'] w
-              ∗ src ↦ᵣ inl z
-              ∗ dst ↦ᵣ inr ((p,g),b,e,a)
-              ∗ a ↦ₐ[p'] inl z }}}.
-   Proof.
-     iIntros (Hinstr Hfl Hfl' Hvpc Hpca' [Hwa Hwb] φ)
-             "(>HPC & >Hi & >Hsrc & >Hdst & >Hsrca) Hφ".
-    iDestruct (map_of_regs_3 with "HPC Hsrc Hdst") as "[Hmap (%&%&%)]".
-    pose proof (writeAllowed_nonO _ _ Hfl' Hwa) as Hp''.
-    pose proof (correctPC_nonO _ _ _ _ _ _ Hfl Hvpc) as Hpc_p'.
-    iDestruct (memMap_resource_2ne_apply with "Hi Hsrca") as "[Hmem %]"; auto.
-
-    iApply (wp_store _ pc_p with "[$Hmap $Hmem]"); eauto; simplify_map_eq; eauto.
-    { by rewrite !dom_insert; set_solver+. }
-    { eapply mem_neq_implies_allow_store_map with (a := a) (p' := p'); eauto.
-      all: by simplify_map_eq. }
-    iNext. iIntros (regs' mem' retv) "(#Hspec & Hmem & Hmap)".
-    iDestruct "Hspec" as %Hspec.
-
-    destruct Hspec as [ | * Hfail ].
-     { (* Success *)
-       iApply "Hφ".
-       destruct H7 as [Hrr2 _]. simplify_map_eq.
-       rewrite insert_commute // insert_insert.
-       iDestruct (memMap_resource_2ne with "Hmem") as "[Hpc_a Ha]";auto.
-       incrementPC_inv.
-       simplify_map_eq.
-       rewrite insert_insert.
-       iDestruct (regs_of_map_3 with "[$Hmap]") as "[HPC [Hsrc Hdst] ]"; eauto. iFrame. }
-     { (* Failure (contradiction) *)
-       destruct Hfail; try incrementPC_inv; simplify_map_eq; eauto.
-       destruct o. all: congruence.
-     }
-   Qed.
-
-    Lemma wp_store_success_reg E pc_p pc_g pc_b pc_e pc_a pc_a' w dst src w'
-         p g b e a w'' pc_p' p' :
+   Lemma wp_store_success_reg E pc_p pc_b pc_e pc_a pc_a' w dst src w'
+         p b e a w'' :
       decodeInstrW w = Store dst (inr src) →
-      PermFlows pc_p pc_p' →
-      PermFlows p p' →
-     isCorrectPC (inr ((pc_p,pc_g),pc_b,pc_e,pc_a)) →
+     isCorrectPC (inr (pc_p,pc_b,pc_e,pc_a)) →
      (pc_a + 1)%a = Some pc_a' →
-     writeAllowed p = true ∧ withinBounds ((p, g), b, e, a) = true →
-     (isLocalWord w'' = false ∨ (p = RWLX ∨ p = RWL)) →
+     writeAllowed p = true ∧ withinBounds (p,b, e, a) = true →
 
-     {{{ ▷ PC ↦ᵣ inr ((pc_p,pc_g),pc_b,pc_e,pc_a)
-           ∗ ▷ pc_a ↦ₐ[pc_p'] w
+     {{{ ▷ PC ↦ᵣ inr (pc_p,pc_b,pc_e,pc_a)
+           ∗ ▷ pc_a ↦ₐ w
            ∗ ▷ src ↦ᵣ w''
-           ∗ ▷ dst ↦ᵣ inr ((p,g),b,e,a)
-           ∗ ▷ a ↦ₐ[p'] w' }}}
+           ∗ ▷ dst ↦ᵣ inr (p,b,e,a)
+           ∗ ▷ a ↦ₐ w' }}}
        Instr Executable @ E
        {{{ RET NextIV;
-           PC ↦ᵣ inr ((pc_p,pc_g),pc_b,pc_e,pc_a')
-              ∗ pc_a ↦ₐ[pc_p'] w
+           PC ↦ᵣ inr (pc_p,pc_b,pc_e,pc_a')
+              ∗ pc_a ↦ₐ w
               ∗ src ↦ᵣ w''
-              ∗ dst ↦ᵣ inr ((p,g),b,e,a)
-              ∗ a ↦ₐ[p'] w'' }}}.
+              ∗ dst ↦ᵣ inr (p,b,e,a)
+              ∗ a ↦ₐ w'' }}}.
     Proof.
-      iIntros (Hinstr Hfl Hfl' Hvpc Hpca' [Hwa Hwb] Hloc φ)
+      iIntros (Hinstr Hvpc Hpca' [Hwa Hwb] φ)
              "(>HPC & >Hi & >Hsrc & >Hdst & >Hsrca) Hφ".
     iDestruct (map_of_regs_3 with "HPC Hsrc Hdst") as "[Hmap (%&%&%)]".
-    pose proof (writeAllowed_nonO _ _ Hfl' Hwa) as Hp''.
-    pose proof (correctPC_nonO _ _ _ _ _ _ Hfl Hvpc) as Hpc_p'.
     iDestruct (memMap_resource_2ne_apply with "Hi Hsrca") as "[Hmem %]"; auto.
 
     iApply (wp_store _ pc_p with "[$Hmap $Hmem]"); eauto; simplify_map_eq; eauto.
     { by rewrite !dom_insert; set_solver+. }
-    { eapply mem_neq_implies_allow_store_map with (a := a) (p' := p'); eauto.
+    { eapply mem_neq_implies_allow_store_map with (a := a); eauto.
       all: by simplify_map_eq. }
     iNext. iIntros (regs' mem' retv) "(#Hspec & Hmem & Hmap)".
     iDestruct "Hspec" as %Hspec.
@@ -826,41 +626,35 @@ Section cap_lang_rules.
      { (* Failure (contradiction) *)
        destruct Hfail; try incrementPC_inv; simplify_map_eq; eauto.
        destruct o. all: try congruence.
-       destruct Hloc as [Hlw | Hpwl]; first congruence. naive_solver.
      }
     Qed.
 
-   Lemma wp_store_success_reg_same E pc_p pc_g pc_b pc_e pc_a pc_a' w dst w'
-         p g b e a pc_p' p' :
+   Lemma wp_store_success_reg_same E pc_p pc_b pc_e pc_a pc_a' w dst w'
+         p b e a :
      decodeInstrW w = Store dst (inr dst) →
-     PermFlows pc_p pc_p' →
-     PermFlows p p' →
-     isCorrectPC (inr ((pc_p,pc_g),pc_b,pc_e,pc_a)) →
+     isCorrectPC (inr (pc_p,pc_b,pc_e,pc_a)) →
      (pc_a + 1)%a = Some pc_a' →
-     writeAllowed p = true ∧ withinBounds ((p, g), b, e, a) = true →
-     (isLocal g = false ∨ (p = RWLX ∨ p = RWL)) →
+     writeAllowed p = true ∧ withinBounds (p, b, e, a) = true →
 
-     {{{ ▷ PC ↦ᵣ inr ((pc_p,pc_g),pc_b,pc_e,pc_a)
-           ∗ ▷ pc_a ↦ₐ[pc_p'] w
-           ∗ ▷ dst ↦ᵣ inr ((p,g),b,e,a)
-           ∗ ▷ a ↦ₐ[p'] w' }}}
+     {{{ ▷ PC ↦ᵣ inr (pc_p,pc_b,pc_e,pc_a)
+           ∗ ▷ pc_a ↦ₐ w
+           ∗ ▷ dst ↦ᵣ inr (p,b,e,a)
+           ∗ ▷ a ↦ₐ w' }}}
        Instr Executable @ E
        {{{ RET NextIV;
-           PC ↦ᵣ inr ((pc_p,pc_g),pc_b,pc_e,pc_a')
-              ∗ pc_a ↦ₐ[pc_p'] w
-              ∗ dst ↦ᵣ inr ((p,g),b,e,a)
-              ∗ a ↦ₐ[p'] inr ((p,g),b,e,a) }}}.
+           PC ↦ᵣ inr (pc_p,pc_b,pc_e,pc_a')
+              ∗ pc_a ↦ₐ w
+              ∗ dst ↦ᵣ inr (p,b,e,a)
+              ∗ a ↦ₐ inr (p,b,e,a) }}}.
    Proof.
-    iIntros (Hinstr Hfl Hfl' Hvpc Hpca' [Hwa Hwb] Hloc φ)
+    iIntros (Hinstr Hvpc Hpca' [Hwa Hwb] φ)
              "(>HPC & >Hi & >Hdst & >Hsrca) Hφ".
     iDestruct (map_of_regs_2 with "HPC Hdst") as "[Hmap %]".
-    pose proof (writeAllowed_nonO _ _ Hfl' Hwa) as Hp''.
-    pose proof (correctPC_nonO _ _ _ _ _ _ Hfl Hvpc) as Hpc_p'.
     iDestruct (memMap_resource_2ne_apply with "Hi Hsrca") as "[Hmem %]"; auto.
 
     iApply (wp_store _ pc_p with "[$Hmap $Hmem]"); eauto; simplify_map_eq; eauto.
     { by rewrite !dom_insert; set_solver+. }
-    { eapply mem_neq_implies_allow_store_map with (a := a) (p' := p'); eauto.
+    { eapply mem_neq_implies_allow_store_map with (a := a); eauto.
       all: by simplify_map_eq. }
     iNext. iIntros (regs' mem' retv) "(#Hspec & Hmem & Hmap)".
     iDestruct "Hspec" as %Hspec.
@@ -878,40 +672,35 @@ Section cap_lang_rules.
      { (* Failure (contradiction) *)
        destruct Hfail; try incrementPC_inv; simplify_map_eq; eauto.
        destruct o. all: try congruence.
-       destruct Hloc as [Hlw | Hpwl]; first congruence. naive_solver.
      }
     Qed.
 
-   Lemma wp_store_success_z E pc_p pc_g pc_b pc_e pc_a pc_a' w dst z w'
-         p g b e a pc_p' p' :
+   Lemma wp_store_success_z E pc_p pc_b pc_e pc_a pc_a' w dst z w'
+         p b e a :
      decodeInstrW w = Store dst (inl z) →
-     PermFlows pc_p pc_p' →
-     PermFlows p p' →
-     isCorrectPC (inr ((pc_p,pc_g),pc_b,pc_e,pc_a)) →
+     isCorrectPC (inr (pc_p,pc_b,pc_e,pc_a)) →
      (pc_a + 1)%a = Some pc_a' →
-     writeAllowed p = true ∧ withinBounds ((p, g), b, e, a) = true →
+     writeAllowed p = true ∧ withinBounds (p, b, e, a) = true →
 
-     {{{ ▷ PC ↦ᵣ inr ((pc_p,pc_g),pc_b,pc_e,pc_a)
-           ∗ ▷ pc_a ↦ₐ[pc_p'] w
-           ∗ ▷ dst ↦ᵣ inr ((p,g),b,e,a)
-           ∗ ▷ a ↦ₐ[p'] w' }}}
+     {{{ ▷ PC ↦ᵣ inr (pc_p,pc_b,pc_e,pc_a)
+           ∗ ▷ pc_a ↦ₐ w
+           ∗ ▷ dst ↦ᵣ inr (p,b,e,a)
+           ∗ ▷ a ↦ₐ w' }}}
        Instr Executable @ E
        {{{ RET NextIV;
-           PC ↦ᵣ inr ((pc_p,pc_g),pc_b,pc_e,pc_a')
-              ∗ pc_a ↦ₐ[pc_p'] w
-              ∗ dst ↦ᵣ inr ((p,g),b,e,a)
-              ∗ a ↦ₐ[p'] inl z }}}.
+           PC ↦ᵣ inr (pc_p,pc_b,pc_e,pc_a')
+              ∗ pc_a ↦ₐ w
+              ∗ dst ↦ᵣ inr (p,b,e,a)
+              ∗ a ↦ₐ inl z }}}.
    Proof.
-     iIntros (Hinstr Hfl Hfl' Hvpc Hpca' [Hwa Hwb] φ)
+     iIntros (Hinstr Hvpc Hpca' [Hwa Hwb] φ)
              "(>HPC & >Hi & >Hdst & >Hsrca) Hφ".
     iDestruct (map_of_regs_2 with "HPC Hdst") as "[Hmap %]".
-    pose proof (writeAllowed_nonO _ _ Hfl' Hwa) as Hp''.
-    pose proof (correctPC_nonO _ _ _ _ _ _ Hfl Hvpc) as Hpc_p'.
     iDestruct (memMap_resource_2ne_apply with "Hi Hsrca") as "[Hmem %]"; auto.
 
     iApply (wp_store _ pc_p with "[$Hmap $Hmem]"); eauto; simplify_map_eq; eauto.
     { by rewrite !dom_insert; set_solver+. }
-    { eapply mem_neq_implies_allow_store_map with (a := a) (p' := p'); eauto.
+    { eapply mem_neq_implies_allow_store_map with (a := a); eauto.
       all: by simplify_map_eq. }
     iNext. iIntros (regs' mem' retv) "(#Hspec & Hmem & Hmap)".
     iDestruct "Hspec" as %Hspec.
