theories/rules/rules_Subseg.v
@@ -5,7 +5,7 @@ From iris.proofmode Require Import tactics.
 From iris.algebra Require Import frac.
 
 Section cap_lang_rules.
-  Context `{memG Σ, regG Σ, MonRef: MonRefG (leibnizO _) CapR_rtc Σ}.
+  Context `{memG Σ, regG Σ}.
   Context `{MachineParameters}.
   Implicit Types P Q : iProp Σ.
   Implicit Types σ : ExecConf.
@@ -19,18 +19,17 @@ Section cap_lang_rules.
   (* TODO: Move somewhere *)
   Ltac destruct_cap c :=
     let p := fresh "p" in
-    let g := fresh "g" in
     let b := fresh "b" in
     let e := fresh "e" in
     let a := fresh "a" in
-    destruct c as ((((p & g) & b) & e) & a).
+    destruct c as (((p & b) & e) & a).
 
   Inductive Subseg_failure  (regs: Reg) (dst: RegName) (src1 src2: Z + RegName) : Reg → Prop :=
   | Subseg_fail_dst_noncap z :
       regs !! dst = Some (inl z) →
       Subseg_failure regs dst src1 src2 regs
-  | Subseg_fail_pE p g b e a :
-      regs !! dst = Some (inr (p, g, b, e, a)) →
+  | Subseg_fail_pE p b e a :
+      regs !! dst = Some (inr (p, b, e, a)) →
       p = E →
       Subseg_failure regs dst src1 src2 regs
   | Subseg_fail_src1_nonaddr :
@@ -39,60 +38,57 @@ Section cap_lang_rules.
   | Subseg_fail_src2_nonaddr :
       addr_of_argument regs src2 = None →
       Subseg_failure regs dst src1 src2 regs
-  | Subseg_fail_not_iswithin p g b e a a1 a2 :
-      regs !! dst = Some (inr (p, g, b, e, a)) →
+  | Subseg_fail_not_iswithin p b e a a1 a2 :
+      regs !! dst = Some (inr (p, b, e, a)) →
       addr_of_argument regs src1 = Some a1 →
       addr_of_argument regs src2 = Some a2 →
       isWithin a1 a2 b e = false →
       Subseg_failure regs dst src1 src2 regs
-  | Subseg_fail_incrPC p g b e a a1 a2 :
-      regs !! dst = Some (inr (p, g, b, e, a)) →
+  | Subseg_fail_incrPC p b e a a1 a2 :
+      regs !! dst = Some (inr (p, b, e, a)) →
       p <> E →
       addr_of_argument regs src1 = Some a1 →
       addr_of_argument regs src2 = Some a2 →
       isWithin a1 a2 b e = true →
-      incrementPC (<[ dst := inr (p, g, a1, a2, a) ]> regs) = None →
-      Subseg_failure regs dst src1 src2 (<[ dst := inr (p, g, a1, a2, a) ]> regs).
+      incrementPC (<[ dst := inr (p, a1, a2, a) ]> regs) = None →
+      Subseg_failure regs dst src1 src2 (<[ dst := inr (p, a1, a2, a) ]> regs).
 
   Inductive Subseg_spec (regs: Reg) (dst: RegName) (src1 src2: Z + RegName) (regs': Reg): cap_lang.val -> Prop :=
-  | Subseg_spec_success p g b e a a1 a2:
-      regs !! dst = Some (inr (p, g, b, e, a)) ->
+  | Subseg_spec_success p b e a a1 a2:
+      regs !! dst = Some (inr (p, b, e, a)) ->
       p <> E ->
       addr_of_argument regs src1 = Some a1 ->
       addr_of_argument regs src2 = Some a2 ->
       isWithin a1 a2 b e = true ->
-      incrementPC (<[ dst := inr (p, g, a1, a2, a) ]> regs) = Some regs' ->
+      incrementPC (<[ dst := inr (p, a1, a2, a) ]> regs) = Some regs' ->
       Subseg_spec regs dst src1 src2 regs' NextIV
   | Subseg_spec_failure :
       Subseg_failure regs dst src1 src2 regs' →
       Subseg_spec regs dst src1 src2 regs' FailedV.
 
   
-  Lemma wp_Subseg Ep pc_p pc_g pc_b pc_e pc_a pc_p' w dst src1 src2 regs :
+  Lemma wp_Subseg Ep pc_p pc_b pc_e pc_a w dst src1 src2 regs :
     decodeInstrW w = Subseg dst src1 src2 ->
-
-    PermFlows pc_p pc_p' →
-    isCorrectPC (inr ((pc_p, pc_g), pc_b, pc_e, pc_a)) →
-    regs !! PC = Some (inr ((pc_p, pc_g), pc_b, pc_e, pc_a)) →
+    isCorrectPC (inr (pc_p, pc_b, pc_e, pc_a)) →
+    regs !! PC = Some (inr (pc_p, pc_b, pc_e, pc_a)) →
     regs_of (Subseg dst src1 src2) ⊆ dom _ regs →
-    {{{ ▷ pc_a ↦ₐ[pc_p'] w ∗
+    
+    {{{ ▷ pc_a ↦ₐ w ∗
         ▷ [∗ map] k↦y ∈ regs, k ↦ᵣ y }}}
       Instr Executable @ Ep
     {{{ regs' retv, RET retv;
         ⌜ Subseg_spec regs dst src1 src2 regs' retv ⌝ ∗
-        pc_a ↦ₐ[pc_p'] w ∗
+        pc_a ↦ₐ w ∗
         [∗ map] k↦y ∈ regs', k ↦ᵣ y }}}.
   Proof.
-    iIntros (Hinstr Hfl Hvpc HPC Dregs φ) "(>Hpc_a & >Hmap) Hφ".
+    iIntros (Hinstr Hvpc HPC Dregs φ) "(>Hpc_a & >Hmap) Hφ".
     iApply wp_lift_atomic_head_step_no_fork; auto.
     iIntros (σ1 l1 l2 n) "Hσ1 /=". destruct σ1; simpl.
     iDestruct "Hσ1" as "[Hr Hm]".
-    assert (pc_p' ≠ O).
-    { destruct pc_p'; auto. destruct pc_p; inversion Hfl. inversion Hvpc; naive_solver. }
     iDestruct (gen_heap_valid_inclSepM with "Hr Hmap") as %Hregs.
     have HPC' := regs_lookup_eq _ _ _ HPC.
     have ? := lookup_weaken _ _ _ _ HPC Hregs.
-    iDestruct (@gen_heap_valid_cap with "Hm Hpc_a") as %Hpc_a; auto.
+    iDestruct (@gen_heap_valid with "Hm Hpc_a") as %Hpc_a; auto.
     iModIntro. iSplitR. by iPureIntro; apply normal_always_head_reducible.
     iNext. iIntros (e2 σ2 efs Hpstep).
     apply prim_step_exec_inv in Hpstep as (-> & -> & (c & -> & Hstep)).
@@ -147,7 +143,7 @@ Section cap_lang_rules.
     eapply addr_of_argument_Some_inv' in Ha2 as [z2 [Hz2 Hz2']]; eauto.
 
     assert ((c, σ2) = if isWithin a1 a2 b e then
-                        updatePC (update_reg (r, m) dst (inr (p, g, a1, a2, a))) else
+                        updatePC (update_reg (r, m) dst (inr (p, a1, a2, a))) else
                         (Failed, (r, m)))
       as Hexec.
     { rewrite -Hstep; clear Hstep. 
@@ -161,7 +157,7 @@ Section cap_lang_rules.
     destruct (isWithin a1 a2 b e) eqn:Hiw; cycle 1.
     { inv Hexec. iFailWP "Hφ" Subseg_fail_not_iswithin. }
 
-    destruct (incrementPC (<[ dst := (inr (p, g, a1, a2, a)) ]> regs)) eqn:HX;
+    destruct (incrementPC (<[ dst := (inr (p, a1, a2, a)) ]> regs)) eqn:HX;
       pose proof HX as H'X; cycle 1.
     { apply incrementPC_fail_updatePC with (m:=m) in HX.
       eapply updatePC_fail_incl with (m':=m) in HX.
@@ -172,7 +168,7 @@ Section cap_lang_rules.
       iFailWP "Hφ" Subseg_fail_incrPC. }
 
     eapply (incrementPC_success_updatePC _ m) in HX
-      as (p' & g' & b' & e' & a'' & a_pc' & HPC'' & Ha_pc' & HuPC & ->).
+      as (p' & g' & b' & e' & a'' & a_pc' & HPC'' & HuPC & ->).
     eapply updatePC_success_incl with (m':=m) in HuPC. 2: by eapply insert_mono; eauto.
     simplify_pair_eq. iFrame.
     iMod ((gen_heap_update_inSepM _ _ dst) with "Hr Hmap") as "[Hr Hmap]"; eauto.
@@ -180,31 +176,29 @@ Section cap_lang_rules.
     iFrame. iApply "Hφ". iFrame. iPureIntro. econstructor; eauto.
   Qed.
 
-  Lemma wp_subseg_success E pc_p pc_g pc_b pc_e pc_a w dst r1 r2 p g b e a n1 n2 a1 a2 pc_p' pc_a' :
+  Lemma wp_subseg_success E pc_p pc_b pc_e pc_a w dst r1 r2 p b e a n1 n2 a1 a2 pc_a' :
     decodeInstrW w = Subseg dst (inr r1) (inr r2) →
-    PermFlows pc_p pc_p' → 
-    isCorrectPC (inr ((pc_p,pc_g),pc_b,pc_e,pc_a)) →
+    isCorrectPC (inr (pc_p,pc_b,pc_e,pc_a)) →
     z_to_addr n1 = Some a1 ∧ z_to_addr n2 = Some a2 →
     p ≠ machine_base.E →
-    dst ≠ PC →
     isWithin a1 a2 b e = true →
     (pc_a + 1)%a = Some pc_a' →
     
-    {{{ ▷ PC ↦ᵣ inr ((pc_p,pc_g),pc_b,pc_e,pc_a)
-        ∗ ▷ pc_a ↦ₐ[pc_p'] w
-        ∗ ▷ dst ↦ᵣ inr ((p,g),b,e,a)
+    {{{ ▷ PC ↦ᵣ inr (pc_p,pc_b,pc_e,pc_a)
+        ∗ ▷ pc_a ↦ₐ w
+        ∗ ▷ dst ↦ᵣ inr (p,b,e,a)
         ∗ ▷ r1 ↦ᵣ inl n1
         ∗ ▷ r2 ↦ᵣ inl n2 }}}
       Instr Executable @ E
       {{{ RET NextIV;
-          PC ↦ᵣ inr ((pc_p,pc_g),pc_b,pc_e,pc_a')
-          ∗ pc_a ↦ₐ[pc_p'] w
+          PC ↦ᵣ inr (pc_p,pc_b,pc_e,pc_a')
+          ∗ pc_a ↦ₐ w
           ∗ r1 ↦ᵣ inl n1
           ∗ r2 ↦ᵣ inl n2
-          ∗ dst ↦ᵣ inr (p, g, a1, a2, a)
+          ∗ dst ↦ᵣ inr (p, a1, a2, a)
       }}}.
   Proof.
-    iIntros (Hinstr Hfl Hvpc [Hn1 Hn2] Hpne Hdstne Hwb Hpc_a' ϕ) "(>HPC & >Hpc_a & >Hdst & >Hr1 & >Hr2) Hφ".
+    iIntros (Hinstr Hvpc [Hn1 Hn2] Hpne Hwb Hpc_a' ϕ) "(>HPC & >Hpc_a & >Hdst & >Hr1 & >Hr2) Hφ".
     iDestruct (map_of_regs_4 with "HPC Hr1 Hr2 Hdst") as "[Hmap (%&%&%&%&%&%)]".
     iApply (wp_Subseg with "[$Hmap Hpc_a]"); eauto; simplify_map_eq; eauto.
     by unfold regs_of; rewrite !dom_insert; set_solver+.
@@ -222,29 +216,27 @@ Section cap_lang_rules.
       all: simplify_map_eq; eauto; congruence. }
   Qed.
 
-  Lemma wp_subseg_success_same E pc_p pc_g pc_b pc_e pc_a w dst r1 p g b e a n1 a1 pc_p' pc_a' :
+  Lemma wp_subseg_success_same E pc_p pc_b pc_e pc_a w dst r1 p b e a n1 a1 pc_a' :
     decodeInstrW w = Subseg dst (inr r1) (inr r1) →
-    PermFlows pc_p pc_p' → 
-    isCorrectPC (inr ((pc_p,pc_g),pc_b,pc_e,pc_a)) →
+    isCorrectPC (inr (pc_p,pc_b,pc_e,pc_a)) →
     z_to_addr n1 = Some a1 →
     p ≠ machine_base.E →
-    dst ≠ PC →
     isWithin a1 a1 b e = true →
     (pc_a + 1)%a = Some pc_a' →
     
-    {{{ ▷ PC ↦ᵣ inr ((pc_p,pc_g),pc_b,pc_e,pc_a)
-        ∗ ▷ pc_a ↦ₐ[pc_p'] w
-        ∗ ▷ dst ↦ᵣ inr ((p,g),b,e,a)
+    {{{ ▷ PC ↦ᵣ inr (pc_p,pc_b,pc_e,pc_a)
+        ∗ ▷ pc_a ↦ₐ w
+        ∗ ▷ dst ↦ᵣ inr (p,b,e,a)
         ∗ ▷ r1 ↦ᵣ inl n1 }}}
       Instr Executable @ E
       {{{ RET NextIV;
-          PC ↦ᵣ inr ((pc_p,pc_g),pc_b,pc_e,pc_a')
-          ∗ pc_a ↦ₐ[pc_p'] w
+          PC ↦ᵣ inr (pc_p,pc_b,pc_e,pc_a')
+          ∗ pc_a ↦ₐ w
           ∗ r1 ↦ᵣ inl n1
-          ∗ dst ↦ᵣ inr (p, g, a1, a1, a)
+          ∗ dst ↦ᵣ inr (p, a1, a1, a)
       }}}.
   Proof.
-    iIntros (Hinstr Hfl Hvpc Hn1 Hpne Hdstne Hwb Hpc_a' ϕ) "(>HPC & >Hpc_a & >Hdst & >Hr1) Hφ".
+    iIntros (Hinstr Hvpc Hn1 Hpne Hwb Hpc_a' ϕ) "(>HPC & >Hpc_a & >Hdst & >Hr1) Hφ".
     iDestruct (map_of_regs_3 with "HPC Hr1 Hdst") as "[Hmap (%&%&%)]".
     iApply (wp_Subseg with "[$Hmap Hpc_a]"); eauto; simplify_map_eq; eauto.
     by unfold regs_of; rewrite !dom_insert; set_solver+.
@@ -262,29 +254,27 @@ Section cap_lang_rules.
       all: simplify_map_eq; eauto; congruence. }
   Qed.
 
-  Lemma wp_subseg_success_l E pc_p pc_g pc_b pc_e pc_a w dst r2 p g b e a n1 n2 a1 a2 pc_p' pc_a' :
+  Lemma wp_subseg_success_l E pc_p pc_b pc_e pc_a w dst r2 p b e a n1 n2 a1 a2 pc_a' :
     decodeInstrW w = Subseg dst (inl n1) (inr r2) →
-    PermFlows pc_p pc_p' → 
-    isCorrectPC (inr ((pc_p,pc_g),pc_b,pc_e,pc_a)) →
+    isCorrectPC (inr (pc_p,pc_b,pc_e,pc_a)) →
     z_to_addr n1 = Some a1 ∧ z_to_addr n2 = Some a2 →
     p ≠ machine_base.E →
-    dst ≠ PC →
     isWithin a1 a2 b e = true →
     (pc_a + 1)%a = Some pc_a' →
     
-    {{{ ▷ PC ↦ᵣ inr ((pc_p,pc_g),pc_b,pc_e,pc_a)
-        ∗ ▷ pc_a ↦ₐ[pc_p'] w
-        ∗ ▷ dst ↦ᵣ inr ((p,g),b,e,a)
+    {{{ ▷ PC ↦ᵣ inr (pc_p,pc_b,pc_e,pc_a)
+        ∗ ▷ pc_a ↦ₐ w
+        ∗ ▷ dst ↦ᵣ inr (p,b,e,a)
         ∗ ▷ r2 ↦ᵣ inl n2 }}}
       Instr Executable @ E
       {{{ RET NextIV;
-          PC ↦ᵣ inr ((pc_p,pc_g),pc_b,pc_e,pc_a')
-          ∗ pc_a ↦ₐ[pc_p'] w
+          PC ↦ᵣ inr (pc_p,pc_b,pc_e,pc_a')
+          ∗ pc_a ↦ₐ w
           ∗ r2 ↦ᵣ inl n2
-          ∗ dst ↦ᵣ inr (p, g, a1, a2, a)
+          ∗ dst ↦ᵣ inr (p, a1, a2, a)
       }}}.
   Proof.
-    iIntros (Hinstr Hfl Hvpc [Hn1 Hn2] Hpne Hdstne Hwb Hpc_a' ϕ) "(>HPC & >Hpc_a & >Hdst & >Hr2) Hφ".
+    iIntros (Hinstr Hvpc [Hn1 Hn2] Hpne Hwb Hpc_a' ϕ) "(>HPC & >Hpc_a & >Hdst & >Hr2) Hφ".
     iDestruct (map_of_regs_3 with "HPC Hr2 Hdst") as "[Hmap (%&%&%)]".
     iApply (wp_Subseg with "[$Hmap Hpc_a]"); eauto; simplify_map_eq; eauto.
     by unfold regs_of; rewrite !dom_insert; set_solver+.
@@ -302,29 +292,27 @@ Section cap_lang_rules.
       all: simplify_map_eq; eauto; congruence. }
   Qed.
 
-  Lemma wp_subseg_success_r E pc_p pc_g pc_b pc_e pc_a w dst r1 p g b e a n1 n2 a1 a2 pc_p' pc_a' :
+  Lemma wp_subseg_success_r E pc_p pc_b pc_e pc_a w dst r1 p b e a n1 n2 a1 a2 pc_a' :
     decodeInstrW w = Subseg dst (inr r1) (inl n2) →
-    PermFlows pc_p pc_p' → 
-    isCorrectPC (inr ((pc_p,pc_g),pc_b,pc_e,pc_a)) →
+    isCorrectPC (inr (pc_p,pc_b,pc_e,pc_a)) →
     z_to_addr n1 = Some a1 ∧ z_to_addr n2 = Some a2 →
     p ≠ machine_base.E →
-    dst ≠ PC →
     isWithin a1 a2 b e = true →
     (pc_a + 1)%a = Some pc_a' →
     
-    {{{ ▷ PC ↦ᵣ inr ((pc_p,pc_g),pc_b,pc_e,pc_a)
-        ∗ ▷ pc_a ↦ₐ[pc_p'] w
-        ∗ ▷ dst ↦ᵣ inr ((p,g),b,e,a)
+    {{{ ▷ PC ↦ᵣ inr (pc_p,pc_b,pc_e,pc_a)
+        ∗ ▷ pc_a ↦ₐ w
+        ∗ ▷ dst ↦ᵣ inr (p,b,e,a)
         ∗ ▷ r1 ↦ᵣ inl n1 }}}
       Instr Executable @ E
       {{{ RET NextIV;
-          PC ↦ᵣ inr ((pc_p,pc_g),pc_b,pc_e,pc_a')
-          ∗ pc_a ↦ₐ[pc_p'] w
+          PC ↦ᵣ inr (pc_p,pc_b,pc_e,pc_a')
+          ∗ pc_a ↦ₐ w
           ∗ r1 ↦ᵣ inl n1
-          ∗ dst ↦ᵣ inr (p, g, a1, a2, a)
+          ∗ dst ↦ᵣ inr (p, a1, a2, a)
       }}}.
   Proof.
-    iIntros (Hinstr Hfl Hvpc [Hn1 Hn2] Hpne Hdstne Hwb Hpc_a' ϕ) "(>HPC & >Hpc_a & >Hdst & >Hr1) Hφ".
+    iIntros (Hinstr Hvpc [Hn1 Hn2] Hpne Hwb Hpc_a' ϕ) "(>HPC & >Hpc_a & >Hdst & >Hr1) Hφ".
     iDestruct (map_of_regs_3 with "HPC Hr1 Hdst") as "[Hmap (%&%&%)]".
     iApply (wp_Subseg with "[$Hmap Hpc_a]"); eauto; simplify_map_eq; eauto.
     by unfold regs_of; rewrite !dom_insert; set_solver+.
@@ -342,27 +330,25 @@ Section cap_lang_rules.
       all: simplify_map_eq; eauto; congruence. }
   Qed.
 
-  Lemma wp_subseg_success_lr E pc_p pc_g pc_b pc_e pc_a w dst p g b e a n1 n2 a1 a2 pc_p' pc_a' :
+  Lemma wp_subseg_success_lr E pc_p pc_b pc_e pc_a w dst p b e a n1 n2 a1 a2 pc_a' :
     decodeInstrW w = Subseg dst (inl n1) (inl n2) →
-    PermFlows pc_p pc_p' → 
-    isCorrectPC (inr ((pc_p,pc_g),pc_b,pc_e,pc_a)) →
+    isCorrectPC (inr (pc_p,pc_b,pc_e,pc_a)) →
     z_to_addr n1 = Some a1 ∧ z_to_addr n2 = Some a2 →
     p ≠ machine_base.E →
-    dst ≠ PC →
     isWithin a1 a2 b e = true →
     (pc_a + 1)%a = Some pc_a' →
     
-    {{{ ▷ PC ↦ᵣ inr ((pc_p,pc_g),pc_b,pc_e,pc_a)
-        ∗ ▷ pc_a ↦ₐ[pc_p'] w
-        ∗ ▷ dst ↦ᵣ inr ((p,g),b,e,a) }}}
+    {{{ ▷ PC ↦ᵣ inr (pc_p,pc_b,pc_e,pc_a)
+        ∗ ▷ pc_a ↦ₐ w
+        ∗ ▷ dst ↦ᵣ inr (p,b,e,a) }}}
       Instr Executable @ E
       {{{ RET NextIV;
-          PC ↦ᵣ inr ((pc_p,pc_g),pc_b,pc_e,pc_a')
-          ∗ pc_a ↦ₐ[pc_p'] w
-          ∗ dst ↦ᵣ inr (p, g, a1, a2, a)
+          PC ↦ᵣ inr (pc_p,pc_b,pc_e,pc_a')
+          ∗ pc_a ↦ₐ w
+          ∗ dst ↦ᵣ inr (p, a1, a2, a)
       }}}.
   Proof.
-    iIntros (Hinstr Hfl Hvpc [Hn1 Hn2] Hpne Hdstne Hwb Hpc_a' ϕ) "(>HPC & >Hpc_a & >Hdst) Hφ".
+    iIntros (Hinstr Hvpc [Hn1 Hn2] Hpne Hwb Hpc_a' ϕ) "(>HPC & >Hpc_a & >Hdst) Hφ".
     iDestruct (map_of_regs_2 with "HPC Hdst") as "[Hmap %]".
     iApply (wp_Subseg with "[$Hmap Hpc_a]"); eauto; simplify_map_eq; eauto.
     by unfold regs_of; rewrite !dom_insert; set_solver+.
@@ -379,28 +365,27 @@ Section cap_lang_rules.
       all: simplify_map_eq; eauto; congruence. }
   Qed.
 
-  Lemma wp_subseg_success_pc E pc_p pc_g pc_b pc_e pc_a w r1 r2 n1 n2 a1 a2 pc_p' pc_a' :
+  Lemma wp_subseg_success_pc E pc_p pc_b pc_e pc_a w r1 r2 n1 n2 a1 a2 pc_a' :
     decodeInstrW w = Subseg PC (inr r1) (inr r2) →
-    PermFlows pc_p pc_p' →
-    isCorrectPC (inr ((pc_p,pc_g),pc_b,pc_e,pc_a)) →
+    isCorrectPC (inr (pc_p,pc_b,pc_e,pc_a)) →
     z_to_addr n1 = Some a1 ∧ z_to_addr n2 = Some a2 →
     pc_p ≠ machine_base.E →
     isWithin a1 a2 pc_b pc_e = true →
     (pc_a + 1)%a = Some pc_a' →
     
-    {{{ ▷ PC ↦ᵣ inr ((pc_p,pc_g),pc_b,pc_e,pc_a)
-        ∗ ▷ pc_a ↦ₐ[pc_p'] w
+    {{{ ▷ PC ↦ᵣ inr (pc_p,pc_b,pc_e,pc_a)
+        ∗ ▷ pc_a ↦ₐ w
         ∗ ▷ r1 ↦ᵣ inl n1
         ∗ ▷ r2 ↦ᵣ inl n2 }}}
       Instr Executable @ E
       {{{ RET NextIV;
-          PC ↦ᵣ inr ((pc_p,pc_g),a1,a2,pc_a')
-          ∗ pc_a ↦ₐ[pc_p'] w
+          PC ↦ᵣ inr (pc_p,a1,a2,pc_a')
+          ∗ pc_a ↦ₐ w
           ∗ r1 ↦ᵣ inl n1
           ∗ r2 ↦ᵣ inl n2
       }}}.
   Proof.
-    iIntros (Hinstr Hfl Hvpc [Hn1 Hn2] Hpne Hwb Hpc_a' ϕ) "(>HPC & >Hpc_a & >Hr1 & >Hr2) Hφ".
+    iIntros (Hinstr Hvpc [Hn1 Hn2] Hpne Hwb Hpc_a' ϕ) "(>HPC & >Hpc_a & >Hr1 & >Hr2) Hφ".
     iDestruct (map_of_regs_3 with "HPC Hr1 Hr2") as "[Hmap (%&%&%)]".
     iApply (wp_Subseg with "[$Hmap Hpc_a]"); eauto; simplify_map_eq; eauto.
     by unfold regs_of; rewrite !dom_insert; set_solver+.
@@ -417,26 +402,25 @@ Section cap_lang_rules.
       all: simplify_map_eq; eauto; try congruence. congruence. }
   Qed.
 
-  Lemma wp_subseg_success_pc_same E pc_p pc_g pc_b pc_e pc_a w r1 n1 a1 pc_p' pc_a' :
+  Lemma wp_subseg_success_pc_same E pc_p pc_b pc_e pc_a w r1 n1 a1 pc_a' :
     decodeInstrW w = Subseg PC (inr r1) (inr r1) →
-    PermFlows pc_p pc_p' →
-    isCorrectPC (inr ((pc_p,pc_g),pc_b,pc_e,pc_a)) →
+    isCorrectPC (inr (pc_p,pc_b,pc_e,pc_a)) →
     z_to_addr n1 = Some a1 →
     pc_p ≠ machine_base.E →
     isWithin a1 a1 pc_b pc_e = true →
     (pc_a + 1)%a = Some pc_a' →
     
-    {{{ ▷ PC ↦ᵣ inr ((pc_p,pc_g),pc_b,pc_e,pc_a)
-        ∗ ▷ pc_a ↦ₐ[pc_p'] w
+    {{{ ▷ PC ↦ᵣ inr (pc_p,pc_b,pc_e,pc_a)
+        ∗ ▷ pc_a ↦ₐ w
         ∗ ▷ r1 ↦ᵣ inl n1 }}}
       Instr Executable @ E
       {{{ RET NextIV;
-          PC ↦ᵣ inr ((pc_p,pc_g),a1,a1,pc_a')
-          ∗ pc_a ↦ₐ[pc_p'] w
+          PC ↦ᵣ inr (pc_p,a1,a1,pc_a')
+          ∗ pc_a ↦ₐ w
           ∗ r1 ↦ᵣ inl n1
       }}}.
   Proof.
-    iIntros (Hinstr Hfl Hvpc Hn1 Hpne Hwb Hpc_a' ϕ) "(>HPC & >Hpc_a & >Hr1) Hφ".
+    iIntros (Hinstr Hvpc Hn1 Hpne Hwb Hpc_a' ϕ) "(>HPC & >Hpc_a & >Hr1) Hφ".
     iDestruct (map_of_regs_2 with "HPC Hr1") as "[Hmap %]".
     iApply (wp_Subseg with "[$Hmap Hpc_a]"); eauto; simplify_map_eq; eauto.
     by unfold regs_of; rewrite !dom_insert; set_solver+.
@@ -453,26 +437,25 @@ Section cap_lang_rules.
       all: simplify_map_eq; eauto; try congruence. congruence. }
   Qed.
 
-  Lemma wp_subseg_success_pc_l E pc_p pc_g pc_b pc_e pc_a w r2 n1 n2 a1 a2 pc_p' pc_a' :
+  Lemma wp_subseg_success_pc_l E pc_p pc_b pc_e pc_a w r2 n1 n2 a1 a2 pc_a' :
     decodeInstrW w = Subseg PC (inl n1) (inr r2) →
-    PermFlows pc_p pc_p' →
-    isCorrectPC (inr ((pc_p,pc_g),pc_b,pc_e,pc_a)) →
+    isCorrectPC (inr (pc_p,pc_b,pc_e,pc_a)) →
     z_to_addr n1 = Some a1 ∧ z_to_addr n2 = Some a2 →
     pc_p ≠ machine_base.E →
     isWithin a1 a2 pc_b pc_e = true →
     (pc_a + 1)%a = Some pc_a' →
     
-    {{{ ▷ PC ↦ᵣ inr ((pc_p,pc_g),pc_b,pc_e,pc_a)
-        ∗ ▷ pc_a ↦ₐ[pc_p'] w
+    {{{ ▷ PC ↦ᵣ inr (pc_p,pc_b,pc_e,pc_a)
+        ∗ ▷ pc_a ↦ₐ w
         ∗ ▷ r2 ↦ᵣ inl n2 }}}
       Instr Executable @ E
       {{{ RET NextIV;
-          PC ↦ᵣ inr ((pc_p,pc_g),a1,a2,pc_a')
-          ∗ pc_a ↦ₐ[pc_p'] w
+          PC ↦ᵣ inr (pc_p,a1,a2,pc_a')
+          ∗ pc_a ↦ₐ w
           ∗ r2 ↦ᵣ inl n2
       }}}.
   Proof.
-    iIntros (Hinstr Hfl Hvpc [Hn1 Hn2] Hpne Hwb Hpc_a' ϕ) "(>HPC & >Hpc_a & >Hr2) Hφ".
+    iIntros (Hinstr Hvpc [Hn1 Hn2] Hpne Hwb Hpc_a' ϕ) "(>HPC & >Hpc_a & >Hr2) Hφ".
     iDestruct (map_of_regs_2 with "HPC Hr2") as "[Hmap %]".
     iApply (wp_Subseg with "[$Hmap Hpc_a]"); eauto; simplify_map_eq; eauto.
     by unfold regs_of; rewrite !dom_insert; set_solver+.
@@ -489,26 +472,25 @@ Section cap_lang_rules.
       all: simplify_map_eq; eauto; try congruence. congruence. }
   Qed.
 
-  Lemma wp_subseg_success_pc_r E pc_p pc_g pc_b pc_e pc_a w r1 n1 n2 a1 a2 pc_p' pc_a' :
+  Lemma wp_subseg_success_pc_r E pc_p pc_b pc_e pc_a w r1 n1 n2 a1 a2 pc_a' :
     decodeInstrW w = Subseg PC (inr r1) (inl n2) →
-    PermFlows pc_p pc_p' →
-    isCorrectPC (inr ((pc_p,pc_g),pc_b,pc_e,pc_a)) →
+    isCorrectPC (inr (pc_p,pc_b,pc_e,pc_a)) →
     z_to_addr n1 = Some a1 ∧ z_to_addr n2 = Some a2 →
     pc_p ≠ machine_base.E →
     isWithin a1 a2 pc_b pc_e = true →
     (pc_a + 1)%a = Some pc_a' →
     
-    {{{ ▷ PC ↦ᵣ inr ((pc_p,pc_g),pc_b,pc_e,pc_a)
-        ∗ ▷ pc_a ↦ₐ[pc_p'] w
+    {{{ ▷ PC ↦ᵣ inr (pc_p,pc_b,pc_e,pc_a)
+        ∗ ▷ pc_a ↦ₐ w
         ∗ ▷ r1 ↦ᵣ inl n1 }}}
       Instr Executable @ E
       {{{ RET NextIV;
-          PC ↦ᵣ inr ((pc_p,pc_g),a1,a2,pc_a')
-          ∗ pc_a ↦ₐ[pc_p'] w
+          PC ↦ᵣ inr (pc_p,a1,a2,pc_a')
+          ∗ pc_a ↦ₐ w
           ∗ r1 ↦ᵣ inl n1
       }}}.
   Proof.
-    iIntros (Hinstr Hfl Hvpc [Hn1 Hn2] Hpne Hwb Hpc_a' ϕ) "(>HPC & >Hpc_a & >Hr1) Hφ".
+    iIntros (Hinstr Hvpc [Hn1 Hn2] Hpne Hwb Hpc_a' ϕ) "(>HPC & >Hpc_a & >Hr1) Hφ".
     iDestruct (map_of_regs_2 with "HPC Hr1") as "[Hmap %]".
     iApply (wp_Subseg with "[$Hmap Hpc_a]"); eauto; simplify_map_eq; eauto.
     by unfold regs_of; rewrite !dom_insert; set_solver+.
@@ -525,24 +507,23 @@ Section cap_lang_rules.
       all: simplify_map_eq; eauto; try congruence. congruence. }
   Qed.
 
-  Lemma wp_subseg_success_pc_lr E pc_p pc_g pc_b pc_e pc_a w n1 n2 a1 a2 pc_p' pc_a' :
+  Lemma wp_subseg_success_pc_lr E pc_p pc_b pc_e pc_a w n1 n2 a1 a2 pc_a' :
     decodeInstrW w = Subseg PC (inl n1) (inl n2) →
-    PermFlows pc_p pc_p' →
-    isCorrectPC (inr ((pc_p,pc_g),pc_b,pc_e,pc_a)) →
+    isCorrectPC (inr (pc_p,pc_b,pc_e,pc_a)) →
     z_to_addr n1 = Some a1 ∧ z_to_addr n2 = Some a2 →
     pc_p ≠ machine_base.E →
     isWithin a1 a2 pc_b pc_e = true →
     (pc_a + 1)%a = Some pc_a' →
     
-    {{{ ▷ PC ↦ᵣ inr ((pc_p,pc_g),pc_b,pc_e,pc_a)
-        ∗ ▷ pc_a ↦ₐ[pc_p'] w }}}
+    {{{ ▷ PC ↦ᵣ inr (pc_p,pc_b,pc_e,pc_a)
+        ∗ ▷ pc_a ↦ₐ w }}}
       Instr Executable @ E
       {{{ RET NextIV;
-          PC ↦ᵣ inr ((pc_p,pc_g),a1,a2,pc_a')
-          ∗ pc_a ↦ₐ[pc_p'] w
+          PC ↦ᵣ inr (pc_p,a1,a2,pc_a')
+          ∗ pc_a ↦ₐ w
       }}}.
   Proof.
-    iIntros (Hinstr Hfl Hvpc [Hn1 Hn2] Hpne Hwb Hpc_a' ϕ) "(>HPC & >Hpc_a) Hφ".
+    iIntros (Hinstr Hvpc [Hn1 Hn2] Hpne Hwb Hpc_a' ϕ) "(>HPC & >Hpc_a) Hφ".
     iDestruct (map_of_regs_1 with "HPC") as "Hmap".
     iApply (wp_Subseg with "[$Hmap Hpc_a]"); eauto; simplify_map_eq; eauto.
     by unfold regs_of; rewrite !dom_insert; set_solver+.
